wordarray WIP: cleaned up files
Shifted the update semantic embeddings of the word array functions and
the related proofs to "WordArray_Update.thy". Shifted the value semantic
embeddings of the word array functions and related proofs to
"WordArray_Value.thy". Shifted the xi abstractions to
"WordArray_UAbsFun.thy" and "WordArray_VAbsFun.thy" for the update and
value semantics respectively.

cogent/examples/wa_connect/WordArray_UpdCCorres.thy
@@ -2,10 +2,12 @@
   This file contains the update semantics to C correspondence lemmas for word array functions
 *)
 theory WordArray_UpdCCorres
-  imports WordArray_Abstractions
+  imports WordArray_UAbsFun
 begin
 
 context WordArray begin
+
+thm abbreviated_type_defs
 (*
 abbreviation "w_val h w \<equiv> values_C (h w)"
 abbreviation "w_len h w \<equiv> SCAST(32 signed \<rightarrow> 32) (len_C (h w))"
@@ -65,9 +67,8 @@ lemma well_typed_related_wordarray: "\<And>\<sigma> st x x' a ts s r w.
 *)
 
 section "Correspondence Lemmas Between Update Semantics and C"
-find_theorems name:".split" -name:"Cogent" -name:"TypeTrackingTyping"
-thm atyp.split
 
+declare \<xi>0.simps[simp del]
 lemma upd_C_wordarray_put2_corres:
   "\<And>i \<gamma> v' \<Gamma>' \<sigma> st.
     \<lbrakk>i < length \<gamma>; val_rel (\<gamma> ! i) v'; \<Gamma>' ! i = option.Some (prod.fst (prod.snd (\<Xi> ''wordarray_put2_0'')))\<rbrakk>
@@ -76,36 +77,37 @@ lemma upd_C_wordarray_put2_corres:
              gets (\<lambda>s. x)
           od)
          \<xi>0 \<gamma> \<Xi> \<Gamma>' \<sigma> st"
-  apply (rule afun_corres; simp)
-  apply (thin_tac "i < length \<gamma>")
-  apply (thin_tac "val_rel (\<gamma> ! i) v'")
+  apply (rule absfun_corres; simp?)
   apply (thin_tac "\<Gamma>' ! i = _")
-  apply (clarsimp simp: abs_rel_def; rename_tac r w)
-  apply (clarsimp simp: val_rel_simp \<Xi>_def wordarray_put2_0_type_def abbreviatedType2_def)
+  apply (clarsimp simp: abs_fun_rel_def; rename_tac r w)
+  apply (rotate_tac -1)
+  apply (subst (asm) \<Xi>_def)
+  apply (subst (asm) \<Xi>_def)
+  apply (clarsimp simp: val_rel_simp wordarray_put2_0_type_def abbreviated_type_defs)
   apply (erule upd.u_t_recE)
   apply (erule upd.u_t_r_consE; clarsimp)+
   apply (erule upd.u_t_primE)+
   apply (subst (asm) lit_type.simps)+
   apply clarsimp
   apply (erule upd.u_t_r_emptyE)
-  apply (erule upd.u_t_p_absE; clarsimp simp: wa_abs_typing_u_def)
-  apply (clarsimp split: atyp.splits type.splits prim_type.splits)
+  apply (erule upd.u_t_p_absE; simp)
+  apply (frule wa_abs_typing_u_elims(1); clarsimp; rename_tac len arr)
   apply (rule conjI)
    apply (monad_eq simp: wordarray_put2_0'_def)
    apply (clarsimp simp: state_rel_def heap_rel_def)
-   apply (erule_tac x = "t2_C.arr_C x'" in allE)
-   apply (erule_tac x = "values_C (heap_WordArray_u32_C st (t2_C.arr_C x')) +\<^sub>p uint (t2_C.idx_C x')" in allE)
+   apply (erule_tac x = "t2_C.arr_C v'" in allE)
+   apply (erule_tac x = "values_C (heap_WordArray_u32_C st (t2_C.arr_C v')) +\<^sub>p uint (t2_C.idx_C v')" in allE)
    apply (clarsimp simp: heap_rel_ptr_def heap_rel_ptr_w32_def wa_abs_repr_def is_valid_simp type_rel_simp)
-   apply (erule_tac x = "t2_C.idx_C x'" in allE)+
+   apply (frule wa_abs_typing_u_elims(5))
+   apply (erule_tac x = "t2_C.idx_C v'" in allE)+
    apply (clarsimp simp: val_rel_simp heap_simp type_rel_simp)
   apply clarsimp
-  apply (rule_tac x = "\<lambda>l. (if \<exists>len arr. (\<sigma> \<circ> ptr_val \<circ> t2_C.arr_C) x' = option.Some (UAbstract (UWA (TPrim (Num U32)) len arr)) \<and> 
-                                l = arr + 4 * t2_C.idx_C x' \<and> t2_C.idx_C x' < len 
-                            then option.Some (UPrim (LU32 (t2_C.val_C x'))) 
+  apply (rule_tac x = "\<lambda>l. (if l = arr + 4 * t2_C.idx_C v' \<and> t2_C.idx_C v' < len 
+                            then option.Some (UPrim (LU32 (t2_C.val_C v'))) 
                             else \<sigma> l)" in exI)
   apply (rule_tac x = "UPtr (ptr_val y') (RCon ''WordArray'' [RPrim (Num U32)])" in exI)
   apply (rule conjI)
-   apply (monad_eq simp: wordarray_put2_0'_def upd_wa_put2_0_def)
+   apply (monad_eq simp: wordarray_put2_0'_def upd_wa_put2_0_def \<xi>0.simps)
   apply (rule conjI)
    apply (rule_tac x = "RCon ''WordArray'' [RPrim (Num U32)]" in exI, simp)
   apply (clarsimp simp: state_rel_def heap_rel_def heap_rel_ptr_meta heap_rel_ptr_w32_meta)
@@ -114,19 +116,19 @@ lemma upd_C_wordarray_put2_corres:
    apply (rule conjI; clarsimp)
     apply (clarsimp simp: type_rel_simp)
    apply (monad_eq simp: wordarray_put2_0'_def)
-   apply (case_tac "idx_C x' < SCAST(32 signed \<rightarrow> 32) (len_C (heap_WordArray_u32_C st (t2_C.arr_C x')))"; 
+   apply (case_tac "idx_C v' < SCAST(32 signed \<rightarrow> 32) (len_C (heap_WordArray_u32_C st (t2_C.arr_C v')))"; 
           drule_tac p = x and uv = uv in all_heap_rel_ptrD; clarsimp simp: is_valid_simp heap_simp)
-  apply (erule_tac x = "t2_C.arr_C x'" in allE)
+  apply (erule_tac x = "t2_C.arr_C v'" in allE)
   apply (clarsimp simp: heap_rel_meta_def wa_abs_repr_def type_rel_simp val_rel_simp)
   apply (monad_eq simp: wordarray_put2_0'_def heap_simp is_valid_simp)
   apply (rule conjI; clarsimp)
-   apply (drule_tac p = "values_C (heap_WordArray_u32_C st (t2_C.arr_C x')) +\<^sub>p uint (t2_C.idx_C x')" and 
+   apply (drule_tac p = "values_C (heap_WordArray_u32_C st (t2_C.arr_C v')) +\<^sub>p uint (t2_C.idx_C v')" and 
                    uv = uv in all_heap_rel_ptrD; clarsimp simp: type_rel_simp val_rel_simp)
   apply (rule conjI)
    apply (clarsimp simp: ptr_add_def)
    apply (metis Ptr_ptr_val mult.commute)
   apply clarsimp
-  apply (case_tac "idx_C x' < SCAST(32 signed \<rightarrow> 32) (len_C (heap_WordArray_u32_C st (t2_C.arr_C x')))";
+  apply (case_tac "idx_C v' < SCAST(32 signed \<rightarrow> 32) (len_C (heap_WordArray_u32_C st (t2_C.arr_C v')))";
          drule_tac p = x and uv = uv in all_heap_rel_ptrD; clarsimp simp: type_rel_simp val_rel_simp)
   done
 
@@ -139,26 +141,27 @@ lemma upd_C_wordarray_length_corres:
              gets (\<lambda>s. x)
           od)
          \<xi>0 \<gamma> \<Xi> \<Gamma>' \<sigma> st"
-  apply (rule afun_corres; simp)
-  apply (clarsimp simp: abs_rel_def; rename_tac r w)
-  apply (thin_tac "i < length \<gamma>")
-  apply (thin_tac "val_rel (\<gamma> ! i) v'")
+  apply (rule absfun_corres; simp?)
+  apply (clarsimp simp: abs_fun_rel_def; rename_tac r w)
   apply (thin_tac "\<Gamma>' ! i = _")
-  apply (clarsimp simp: val_rel_simp \<Xi>_def wordarray_length_0_type_def)
-  apply (erule upd.u_t_p_absE; clarsimp simp: wa_abs_typing_u_def)
-  apply (clarsimp split: atyp.splits type.splits prim_type.splits)
+  apply (rotate_tac -1)
+  apply (subst (asm) \<Xi>_def)
+  apply (subst (asm) \<Xi>_def)
+  apply (clarsimp simp: val_rel_simp wordarray_length_0_type_def)
+  apply (erule upd.u_t_p_absE; simp)
+  apply (frule wa_abs_typing_u_elims(1); clarsimp; rename_tac len arr)
   apply (rule conjI)
    apply (monad_eq simp: wordarray_length_0'_def)
    apply (clarsimp simp: state_rel_def heap_rel_def)
-   apply (erule_tac x = x' in allE)
+   apply (erule_tac x = v' in allE)
    apply (clarsimp simp: heap_rel_ptr_def type_rel_simp wa_abs_repr_def is_valid_simp)
   apply clarsimp
   apply (rule_tac x = \<sigma> in exI)
   apply (rule conjI)
-   apply (clarsimp simp: upd_wa_length_0_def)
+   apply (clarsimp simp: upd_wa_length_0_def \<xi>0.simps)
    apply (monad_eq simp: wordarray_length_0'_def)
    apply (clarsimp simp: state_rel_def heap_rel_def)
-   apply (erule_tac x = x' in allE)
+   apply (erule_tac x = v' in allE)
    apply (clarsimp simp: heap_rel_ptr_def type_rel_simp wa_abs_repr_def heap_simp val_rel_simp)
   apply (monad_eq simp: wordarray_length_0'_def)
   done
@@ -172,44 +175,49 @@ lemma upd_C_wordarray_get_corres:
              gets (\<lambda>s. x)
           od)
          \<xi>0 \<gamma> \<Xi> \<Gamma>' \<sigma> st"
-  apply (rule afun_corres; simp)
-  apply (clarsimp simp: abs_rel_def; rename_tac r w)
-  apply (thin_tac "i < length \<gamma>")
-  apply (thin_tac "val_rel (\<gamma> ! i) v'")
+  apply (rule absfun_corres; simp?)
+  apply (clarsimp simp: abs_fun_rel_def; rename_tac r w)
   apply (thin_tac "\<Gamma>' ! i = _")
-  apply (clarsimp simp: val_rel_simp \<Xi>_def wordarray_get_0_type_def abbreviatedType3_def)
+  apply (rotate_tac -1)
+  apply (subst (asm) \<Xi>_def)
+  apply (subst (asm) \<Xi>_def)
+  apply (clarsimp simp: val_rel_simp wordarray_get_0_type_def abbreviated_type_defs)
   apply (erule upd.u_t_recE)
   apply (erule upd.u_t_r_consE; clarsimp)+
   apply (erule upd.u_t_r_emptyE)
   apply (erule upd.u_t_primE; subst (asm) lit_type.simps; clarsimp)
-  apply (erule upd.u_t_p_absE; clarsimp simp: wa_abs_typing_u_def)
-  apply (clarsimp split: atyp.splits type.splits prim_type.splits)
+  apply (erule upd.u_t_p_absE; simp)
+  apply (frule wa_abs_typing_u_elims(1); clarsimp; rename_tac len arr)
   apply (rule conjI)
    apply (monad_eq simp: wordarray_get_0'_def)
    apply (clarsimp simp: state_rel_def heap_rel_def heap_rel_ptr_meta heap_rel_ptr_w32_meta)
-   apply (drule_tac p = "t1_C.p1_C x'" and uv = "UAbstract (UWA (TPrim (Num U32)) x12 x13)" in all_heap_rel_ptrD; 
+   apply (drule_tac p = "t1_C.p1_C v'" and uv = "UAbstract (UWA (TPrim (Num U32)) len arr)" in all_heap_rel_ptrD; 
           clarsimp simp: type_rel_simp wa_abs_repr_def val_rel_simp is_valid_simp heap_simp)
    apply (drule not_le_imp_less)
-   apply (erule_tac x = "t1_C.p2_C x'" in allE; clarsimp)
-   apply (drule_tac p = "values_C (heap_WordArray_u32_C st (t1_C.p1_C x')) +\<^sub>p uint (t1_C.p2_C x')" and
+   apply (frule wa_abs_typing_u_elims(5))
+   apply (erule_tac x = "t1_C.p2_C v'" in allE; clarsimp)
+   apply (drule_tac p = "values_C (heap_WordArray_u32_C st (t1_C.p1_C v')) +\<^sub>p uint (t1_C.p2_C v')" and
                    uv = "UPrim x" in all_heap_rel_ptrD; simp add: type_rel_simp)
   apply clarsimp
   apply (rule_tac x = \<sigma> in exI)
   apply (rule conjI)
-   apply (clarsimp simp: upd_wa_get_0_def)
-   apply (erule_tac x = "t1_C.p2_C x'" in allE)
+   apply (clarsimp simp: upd_wa_get_0_def \<xi>0.simps)
+   apply (frule wa_abs_typing_u_elims(5))
+   apply (erule_tac x = "t1_C.p2_C v'" in allE)
    apply (monad_eq simp: wordarray_get_0'_def word_less_nat_alt word_le_nat_alt)
    apply (clarsimp simp: state_rel_def heap_rel_def heap_rel_ptr_meta heap_rel_ptr_w32_meta)
-   apply (drule_tac p = "t1_C.p1_C x'" and uv = "UAbstract (UWA (TPrim (Num U32)) x12 x13)" in all_heap_rel_ptrD; 
+   apply (drule_tac p = "t1_C.p1_C v'" and uv = "UAbstract (UWA (TPrim (Num U32)) len arr)" in all_heap_rel_ptrD; 
           clarsimp simp: type_rel_simp wa_abs_repr_def val_rel_simp is_valid_simp heap_simp)
-   apply (drule_tac p = "values_C (heap_WordArray_u32_C st (t1_C.p1_C x')) +\<^sub>p uint (t1_C.p2_C x')" and
+   apply (drule_tac p = "values_C (heap_WordArray_u32_C st (t1_C.p1_C v')) +\<^sub>p uint (t1_C.p2_C v')" and
                    uv = "UPrim x" in all_heap_rel_ptrD;
           clarsimp simp: type_rel_simp val_rel_simp)
   apply (monad_eq simp: wordarray_get_0'_def)
   apply blast
   done
 thm corres_sum corres_app_concrete
-lemma
+declare \<xi>1.simps [simp del]
+(*
+lemma upd_C_wordarray_fold_no_break_corres:
 " \<And>v' i \<gamma> \<Gamma>' \<sigma> s.
     \<lbrakk>i < length \<gamma>; val_rel (\<gamma> ! i) v';
      \<Gamma>' ! i = option.Some (prod.fst (prod.snd (\<Xi> ''wordarray_fold_no_break_0'')))\<rbrakk>
@@ -218,20 +226,20 @@ lemma
 gets (\<lambda>s. x)
                                                                 od)
          \<xi>1 \<gamma> \<Xi>  \<Gamma>' \<sigma> s"
-  apply (rule afun_corres; clarsimp)
-  apply (clarsimp simp: abs_rel_def')
-  apply (thin_tac "i < length \<gamma>")
-  apply (thin_tac "val_rel (\<gamma> ! i) v'")
+  apply (rule absfun_corres; simp?)
+  apply (clarsimp simp: abs_fun_rel_def')
   apply (thin_tac "\<Gamma>' ! i = _")
   apply clarsimp
   apply (clarsimp simp: val_rel_simp)
   apply (erule upd.u_t_recE)
-  apply (clarsimp simp: \<Xi>_def wordarray_fold_no_break_0_type_def abbreviatedType1_def)
+  apply (rotate_tac -3)
+  apply (subst (asm) \<Xi>_def)
+  apply (clarsimp simp: wordarray_fold_no_break_0_type_def abbreviated_type_defs)
   apply (erule upd.u_t_r_consE; clarsimp)+
   apply (erule upd.u_t_primE; subst (asm) lit_type.simps; clarsimp)+
   apply (erule upd.u_t_r_emptyE)
   apply (erule upd.u_t_unitE)
-  apply (case_tac "sint (t5_C.f_C x') \<noteq> sint FUN_ENUM_mul \<and> sint (t5_C.f_C x') \<noteq> sint FUN_ENUM_sum")
+  apply (case_tac "sint (t5_C.f_C v') \<noteq> sint FUN_ENUM_mul \<and> sint (t5_C.f_C v') \<noteq> sint FUN_ENUM_sum")
    apply (clarsimp simp: cogent_function_val_rel
                          FUN_ENUM_sum_def
                          FUN_ENUM_mul_def
@@ -246,8 +254,8 @@ gets (\<lambda>s. x)
                          FUN_ENUM_wordarray_put2_u32_def)
    apply (rule FalseE) 
    apply (thin_tac "_ \<in> state_rel")
-   apply (thin_tac "t5_C.f_C x' \<noteq> 0")
-   apply (thin_tac "sint (t5_C.f_C x') \<noteq> 2")
+   apply (thin_tac "t5_C.f_C v' \<noteq> 0")
+   apply (thin_tac "sint (t5_C.f_C v') \<noteq> 2")
    apply (thin_tac "upd.uval_typing _ _ (UPtr _ _) _ _ _")
    apply (thin_tac "_ = _")+
    apply clarsimp
@@ -260,14 +268,14 @@ gets (\<lambda>s. x)
       apply (erule upd.u_t_afunE; clarsimp)
       apply (clarsimp simp: subtyping_simps(4) 
                             subtyping.simps[of _ _ "TPrim (Num U32)", simplified]
-                            wordarray_get_0_type_def abbreviatedType3_def
-                            subtyping_simps(6))
+                            wordarray_get_0_type_def abbreviated_type_defs
+                            subtyping_simps(6) \<Xi>_def)
      apply (erule disjE)
       apply clarsimp
       apply (erule upd.u_t_afunE; clarsimp)
       apply (clarsimp simp: subtyping_simps(4) 
                             subtyping.simps[of _ _ "TPrim (Num U32)", simplified]
-                            wordarray_put2_0_type_def)
+                            wordarray_put2_0_type_def \<Xi>_def)
      apply (erule disjE)
       apply clarsimp
       apply (erule upd.u_t_funE'; clarsimp)
@@ -281,7 +289,7 @@ gets (\<lambda>s. x)
       apply (erule typing_letE)
       apply (erule typing_appE)
       apply (erule typing_afunE)
-      apply (clarsimp simp: wordarray_get_0_type_def abbreviatedType3_def)
+      apply (clarsimp simp: wordarray_get_0_type_def abbreviated_type_defs \<Xi>_def)
       apply (erule typing_varE)+
       apply (clarsimp simp: split_conv_all_nth weakening_conv_all_nth empty_def)
       apply (erule_tac x = 0 in allE)+
@@ -293,7 +301,7 @@ gets (\<lambda>s. x)
       apply (clarsimp simp: subtyping_simps(4) 
                             subtyping.simps[of _ _ "TPrim (Num U32)", simplified]
                             subtyping.simps[of _ "TRecord _ _ ", simplified]
-                            wordarray_length_0_type_def)
+                            wordarray_length_0_type_def \<Xi>_def)
      apply (erule disjE)
       apply clarsimp
       apply (erule upd.u_t_funE'; clarsimp)
@@ -307,7 +315,7 @@ gets (\<lambda>s. x)
       apply (erule typing_letE)
       apply (erule typing_appE)
       apply (erule typing_afunE)
-      apply (clarsimp simp: wordarray_put2_0_type_def abbreviatedType5_def)
+      apply (clarsimp simp: wordarray_put2_0_type_def abbreviated_type_defs \<Xi>_def)
      apply (erule disjE)
       apply clarsimp
       apply (erule upd.u_t_funE'; clarsimp)
@@ -321,7 +329,7 @@ gets (\<lambda>s. x)
       apply (erule typing_letE)
       apply (erule typing_appE)
       apply (erule typing_afunE)
-      apply (clarsimp simp: wordarray_length_0_type_def)
+      apply (clarsimp simp: wordarray_length_0_type_def \<Xi>_def)
       apply (erule typing_varE)+
       apply (clarsimp simp: split_conv_all_nth weakening_conv_all_nth empty_def)
       apply (erule_tac x = 0 in allE)+
@@ -331,7 +339,8 @@ gets (\<lambda>s. x)
      apply (erule upd.u_t_afunE; clarsimp)
      apply (clarsimp simp: subtyping_simps(4) 
                            subtyping.simps[of _ _ "TPrim (Num U32)", simplified]
-                           subtyping.simps[of _ "TRecord _ _ ", simplified])
+                           subtyping.simps[of _ "TRecord _ _ ", simplified]
+                           \<Xi>_def wordarray_fold_no_break_0_type_def)
     apply clarsimp
     apply (erule upd.u_t_funE')
     apply (clarsimp simp: subtyping_simps(4) 
@@ -349,7 +358,7 @@ gets (\<lambda>s. x)
     apply (erule typing_appE)
     apply (erule typing_afunE)
     apply (erule typing_varE)
-    apply (clarsimp simp: wordarray_length_0_type_def)
+    apply (clarsimp simp: wordarray_length_0_type_def \<Xi>_def)
     apply (frule split_length; simp)
     apply (drule same_type_as_weakened; simp?)
     apply (drule split_preservation_some_left; simp?)
@@ -375,7 +384,7 @@ gets (\<lambda>s. x)
    apply (erule typing_appE)
    apply (erule typing_afunE)
    apply (erule typing_varE)
-   apply (clarsimp simp: wordarray_length_0_type_def)
+   apply (clarsimp simp: wordarray_length_0_type_def \<Xi>_def)
    apply (frule split_length; simp)
    apply (drule same_type_as_weakened; simp?)
    apply (drule split_preservation_some_left; simp?)
@@ -386,24 +395,24 @@ gets (\<lambda>s. x)
    apply clarsimp
   apply clarsimp
   apply (erule upd.u_t_p_absE; clarsimp)
-  apply (clarsimp simp: wordarray_fold_no_break_0'_def upd_wa_foldnb_0_def)
+  apply (clarsimp simp: wordarray_fold_no_break_0'_def upd_wa_foldnb_def \<xi>1.simps)
   apply (subst unknown_bind_ignore)+
   apply clarsimp
   apply wp 
       apply (clarsimp simp: split_def unknown_bind_ignore)
       apply (subst whileLoop_add_inv
-              [where M = "\<lambda>((_, r), _). unat (t5_C.to_C x') - unat r" and 
+              [where M = "\<lambda>((_, r), _). unat (t5_C.to_C v') - unat r" and 
                      I = "\<lambda>(a, b) s. 
-                        (\<exists>func. cogent_function_val_rel x (sint (t5_C.f_C x')) \<and> func = x \<and>
+                        (\<exists>func. cogent_function_val_rel x (sint (t5_C.f_C v')) \<and> func = x \<and>
                         is_uval_fun func \<and> (\<Xi>, [], [option.Some abbreviatedType1] \<turnstile> 
                           (App (uvalfun_to_exprfun func) (Var 0)) : TPrim (Num U32)) \<and>
-                        upd_wa_foldnb_bod \<xi>0 \<sigma> (ptr_val (t5_C.arr_C x')) (t5_C.frm_C x') b 
-                          (uvalfun_to_exprfun func) (UPrim (LU32 (t5_C.acc_C x'))) UUnit {} 
+                        upd_wa_foldnb_bod \<xi>0 \<sigma> (ptr_val (t5_C.arr_C v')) (t5_C.frm_C v') b 
+                          (uvalfun_to_exprfun func) (UPrim (LU32 (t5_C.acc_C v'))) UUnit {} 
                           (\<sigma>, UPrim (LU32 (t3_C.acc_C a)))) \<and> 
-                        (\<sigma>, s) \<in> state_rel \<and> t5_C.frm_C x' \<le> b \<and>
-                        ret = min (t5_C.to_C x') ((SCAST(32 signed \<rightarrow> 32))(len_C (heap_WordArray_u32_C s (t5_C.arr_C x')))) \<and>
-                        (t5_C.frm_C x' \<le> ret \<longrightarrow> b \<le> ret) \<and> (t5_C.frm_C x' \<ge> ret \<longrightarrow> b = t5_C.frm_C x')"])
-      apply (wp; clarsimp simp: split_def unknown_bind_ignore simp del: \<xi>0.simps)
+                        (\<sigma>, s) \<in> state_rel \<and> t5_C.frm_C v' \<le> b \<and>
+                        ret = min (t5_C.to_C v') ((SCAST(32 signed \<rightarrow> 32))(len_C (heap_WordArray_u32_C s (t5_C.arr_C v')))) \<and>
+                        (t5_C.frm_C v' \<le> ret \<longrightarrow> b \<le> ret) \<and> (t5_C.frm_C v' \<ge> ret \<longrightarrow> b = t5_C.frm_C v')"])
+      apply (wp; clarsimp simp: split_def unknown_bind_ignore)
            apply (clarsimp simp: split_def dispatch_t4'_def unknown_bind_ignore)
            apply wp
             apply (clarsimp simp: mul'_def unknown_bind_ignore)
@@ -424,23 +433,22 @@ gets (\<lambda>s. x)
                              FUN_ENUM_wordarray_fold_no_break_0_def
                              FUN_ENUM_wordarray_get_u32_def
                              FUN_ENUM_wordarray_length_u32_def
-                             FUN_ENUM_wordarray_put2_u32_def
-                   simp del: \<xi>0.simps)
+                             FUN_ENUM_wordarray_put2_u32_def)
        apply (thin_tac "upd.uval_typing _ _ _ _ _ _")
        apply (clarsimp simp: wa_abs_typing_u_def)
        apply (thin_tac "_ \<in> state_rel")
        apply (clarsimp split: atyp.splits type.splits prim_type.splits)
        apply (erule_tac x = b in allE)
        apply (clarsimp simp: state_rel_def heap_rel_def heap_rel_ptr_meta heap_rel_ptr_w32_meta)
-       apply (drule_tac p = "t5_C.arr_C x'" and uv = "UAbstract (UWA (TPrim (Num U32)) x12 x13)" in all_heap_rel_ptrD; 
+       apply (drule_tac p = "t5_C.arr_C v'" and uv = "UAbstract (UWA (TPrim (Num U32)) x12 x13)" in all_heap_rel_ptrD; 
               clarsimp simp: type_rel_simps is_valid_simp heap_simp wa_abs_repr_def val_rel_simps) 
-       apply (drule_tac p = "values_C (heap_WordArray_u32_C s (t5_C.arr_C x')) +\<^sub>p uint b" and 
+       apply (drule_tac p = "values_C (heap_WordArray_u32_C sa (t5_C.arr_C v')) +\<^sub>p uint b" and 
                        uv = "UPrim xa" in all_heap_rel_ptrD; clarsimp simp: type_rel_simps)
        apply (rule conjI; clarsimp)
         apply (rule conjI)
          apply (rule_tac r = "UPrim (LU32 (t3_C.acc_C aa))" and 
-                       len = "(SCAST(32 signed \<rightarrow> 32) (len_C (heap_WordArray_u32_C s (t5_C.arr_C x'))))" and
-                       arr = "(ptr_val (values_C (heap_WordArray_u32_C s (t5_C.arr_C x'))))" and
+                       len = "(SCAST(32 signed \<rightarrow> 32) (len_C (heap_WordArray_u32_C sa (t5_C.arr_C v'))))" and
+                       arr = "(ptr_val (values_C (heap_WordArray_u32_C sa (t5_C.arr_C v'))))" and
                          v = "UPrim xa" and \<sigma> = \<sigma> and \<sigma>' = \<sigma> and \<sigma>'' = \<sigma> and ?w1.0 = "{}" and 
                          ?w2.0 = "{}"
                        in upd_wa_foldnb_bod_step; simp?)
@@ -492,8 +500,8 @@ gets (\<lambda>s. x)
         apply (metis (no_types, hide_lams) add.commute diff_less_mono2 max_word_max unat_mono word_Suc_le word_le_less_eq word_less_nat_alt word_not_le)
        apply (rule conjI)
         apply (rule_tac r = "UPrim (LU32 (t3_C.acc_C aa))" and 
-                      len = "(SCAST(32 signed \<rightarrow> 32) (len_C (heap_WordArray_u32_C s (t5_C.arr_C x'))))" and
-                      arr = "(ptr_val (values_C (heap_WordArray_u32_C s (t5_C.arr_C x'))))" and
+                      len = "(SCAST(32 signed \<rightarrow> 32) (len_C (heap_WordArray_u32_C sa (t5_C.arr_C v'))))" and
+                      arr = "(ptr_val (values_C (heap_WordArray_u32_C sa (t5_C.arr_C v'))))" and
                         v = "UPrim xa" and \<sigma> = \<sigma> and \<sigma>' = \<sigma> and \<sigma>'' = \<sigma> and ?w1.0 = "{}" and
                         ?w2.0 = "{}"
                       in upd_wa_foldnb_bod_step; simp?)
@@ -548,7 +556,7 @@ gets (\<lambda>s. x)
       apply (clarsimp simp: state_rel_def heap_rel_def heap_rel_ptr_meta heap_rel_ptr_w32_meta)
       apply (rule_tac x = \<sigma> in exI; clarsimp?)
       apply (rule conjI; clarsimp?)
-      apply (drule_tac p = "t5_C.arr_C x'" and uv = "UAbstract (UWA (TPrim (Num U32)) x12 x13)" in all_heap_rel_ptrD; 
+      apply (drule_tac p = "t5_C.arr_C v'" and uv = "UAbstract (UWA (TPrim (Num U32)) x12 x13)" in all_heap_rel_ptrD; 
              clarsimp simp: type_rel_simps is_valid_simp heap_simp wa_abs_repr_def val_rel_simps) 
       apply (thin_tac "cogent_function_val_rel _ _")
       apply (thin_tac "upd.uval_typing _ _ _ _ _ _")
@@ -565,22 +573,22 @@ gets (\<lambda>s. x)
       apply (rule conjI)
        apply (rule upd.u_t_unit)
       apply (clarsimp simp: \<Xi>_def abbreviatedType1_def wordarray_fold_no_break_0_type_def)
-      apply (case_tac "t5_C.to_C x' = b"; clarsimp?)
-      apply (case_tac "b < t5_C.to_C x'"; clarsimp)
+      apply (case_tac "t5_C.to_C v' = b"; clarsimp?)
+      apply (case_tac "b < t5_C.to_C v'"; clarsimp)
        apply (case_tac x; clarsimp)
-        apply (drule_tac arr = "ptr_val (values_C (heap_WordArray_u32_C s (t5_C.arr_C x')))" and 
-                         len = "SCAST(32 signed \<rightarrow> 32) (len_C (heap_WordArray_u32_C s (t5_C.arr_C x')))" 
+        apply (drule_tac arr = "ptr_val (values_C (heap_WordArray_u32_C sa (t5_C.arr_C v')))" and 
+                         len = "SCAST(32 signed \<rightarrow> 32) (len_C (heap_WordArray_u32_C sa (t5_C.arr_C v')))" 
                          in upd_wa_foldnb_bod_to_geq_lenD; simp?)
-        apply (rule_tac arr = "ptr_val (values_C (heap_WordArray_u32_C s (t5_C.arr_C x')))" and 
-                        len = "SCAST(32 signed \<rightarrow> 32) (len_C (heap_WordArray_u32_C s (t5_C.arr_C x')))" 
+        apply (rule_tac arr = "ptr_val (values_C (heap_WordArray_u32_C sa (t5_C.arr_C v')))" and 
+                        len = "SCAST(32 signed \<rightarrow> 32) (len_C (heap_WordArray_u32_C sa (t5_C.arr_C v')))" 
                         in upd_wa_foldnb_bod_to_geq_len; simp)
-       apply (drule_tac arr = "ptr_val (values_C (heap_WordArray_u32_C s (t5_C.arr_C x')))" and 
-                        len = "SCAST(32 signed \<rightarrow> 32) (len_C (heap_WordArray_u32_C s (t5_C.arr_C x')))" 
+       apply (drule_tac arr = "ptr_val (values_C (heap_WordArray_u32_C sa (t5_C.arr_C v')))" and 
+                        len = "SCAST(32 signed \<rightarrow> 32) (len_C (heap_WordArray_u32_C sa (t5_C.arr_C v')))" 
                         in upd_wa_foldnb_bod_to_geq_lenD; simp?)
-       apply (rule_tac arr = "ptr_val (values_C (heap_WordArray_u32_C s (t5_C.arr_C x')))" and 
-                       len = "SCAST(32 signed \<rightarrow> 32) (len_C (heap_WordArray_u32_C s (t5_C.arr_C x')))" 
+       apply (rule_tac arr = "ptr_val (values_C (heap_WordArray_u32_C sa (t5_C.arr_C v')))" and 
+                       len = "SCAST(32 signed \<rightarrow> 32) (len_C (heap_WordArray_u32_C sa (t5_C.arr_C v')))" 
                        in upd_wa_foldnb_bod_to_geq_len; simp)
-      apply (case_tac "min (t5_C.to_C x') (SCAST(32 signed \<rightarrow> 32) (len_C (heap_WordArray_u32_C s (t5_C.arr_C x')))) \<le> t5_C.frm_C x'")
+      apply (case_tac "min (t5_C.to_C v') (SCAST(32 signed \<rightarrow> 32) (len_C (heap_WordArray_u32_C sa (t5_C.arr_C v')))) \<le> t5_C.frm_C v'")
        apply clarsimp
        apply (case_tac x; clarsimp)
         apply (erule upd_wa_foldnb_bod.elims; clarsimp)
@@ -618,7 +626,7 @@ gets (\<lambda>s. x)
    apply clarsimp
    apply (clarsimp simp: state_rel_def heap_rel_def heap_rel_ptr_meta wa_abs_typing_u_def)
    apply (clarsimp split: atyp.splits type.splits prim_type.splits)
-   apply (drule_tac p = "t5_C.arr_C x'" and uv = "UAbstract (UWA (TPrim (Num U32)) x12 x13)" in all_heap_rel_ptrD;
+   apply (drule_tac p = "t5_C.arr_C v'" and uv = "UAbstract (UWA (TPrim (Num U32)) x12 x13)" in all_heap_rel_ptrD;
           clarsimp simp: wa_abs_repr_def type_rel_simps is_valid_simp)
    apply (thin_tac "upd.uval_typing _ _ _ _ _ _")
    apply (thin_tac "is_valid_WordArray_u32_C _ _")
@@ -706,5 +714,210 @@ gets (\<lambda>s. x)
   apply (erule disjE; clarsimp)
   done
 thm corres_sum corres_app_concrete
+
+lemma 
+" \<And>v' i \<gamma> \<Gamma> \<sigma> s.
+        \<lbrakk>f_C v' = FUN_ENUM_mul; i < length \<gamma>; val_rel (\<gamma> ! i) v';
+         \<Gamma> ! i =
+         option.Some
+          (prod.fst
+            (prod.snd
+              (assoc_lookup
+                [(''wordarray_get_0'', wordarray_get_0_type), (''wordarray_length_0'', wordarray_length_0_type),
+                 (''wordarray_put2_0'', wordarray_put2_0_type), (''wordarray_fold_no_break_0'', wordarray_fold_no_break_0_type),
+                 (''wordarray_get_u32'', Generated_TypeProof.wordarray_get_u32_type),
+                 (''wordarray_length_u32'', Generated_TypeProof.wordarray_length_u32_type),
+                 (''wordarray_put2_u32'', Generated_TypeProof.wordarray_put2_u32_type), (''mul'', Generated_TypeProof.mul_type),
+                 (''mul_arr'', Generated_TypeProof.mul_arr_type), (''sum'', Generated_TypeProof.sum_type),
+                 (''sum_arr'', Generated_TypeProof.sum_arr_type)]
+                ([], TUnit, TUnit) ''wordarray_fold_no_break_0'')))\<rbrakk>
+        \<Longrightarrow> update_sem_init.corres wa_abs_typing_u wa_abs_repr (Generated.state_rel wa_abs_repr)
+             (App (AFun ''wordarray_fold_no_break_0'' []) (Var i)) (do x <- wordarray_fold_no_break_0' v';
+      gets (\<lambda>s. x)
+   od)
+             \<xi>1 \<gamma>
+             (assoc_lookup
+               [(''wordarray_get_0'', wordarray_get_0_type), (''wordarray_length_0'', wordarray_length_0_type),
+                (''wordarray_put2_0'', wordarray_put2_0_type), (''wordarray_fold_no_break_0'', wordarray_fold_no_break_0_type),
+                (''wordarray_get_u32'', Generated_TypeProof.wordarray_get_u32_type),
+                (''wordarray_length_u32'', Generated_TypeProof.wordarray_length_u32_type),
+                (''wordarray_put2_u32'', Generated_TypeProof.wordarray_put2_u32_type), (''mul'', Generated_TypeProof.mul_type),
+                (''mul_arr'', Generated_TypeProof.mul_arr_type), (''sum'', Generated_TypeProof.sum_type),
+                (''sum_arr'', Generated_TypeProof.sum_arr_type)]
+               ([], TUnit, TUnit))
+             \<Gamma> \<sigma> s"
+  
+  by (drule_tac ?\<Gamma>' = \<Gamma> and \<sigma> = \<sigma> and s = s in upd_C_wordarray_fold_no_break_corres[simplified]; simp add: \<Xi>_def)
+ *)
+(*
+High level:
+  * Cogent is a language which eases proving things
+    (ASPLOS Paper: we verified Cogent shallow embedding up to a function spec and it was easy)
+  * Can't do everything in Cogent
+    (No iteration or recursion,
+     linear type system enforces restrictions which are too strict sometimes
+        TODO: 
+          Find examples:
+            - vnode pointers in FS file tables esp. if things like dup2 or Linux fork semantic are
+              implemented (i.e. multiple references to the same vnode)
+            -
+          Note here that the C foreign functions  have to respect the type system + frame
+          Easy in C but hard/impossible in Cogent due to linear types but still respects type system and frame
+    ) 
+  * We have an FFI to C
+    (Introduced in ICFP paper with no examples or verification work)
+  * Amortise C verification cost
+    (Intuitive because of ADT reuse, assuming the ssumptions about the C functions are all provable in a reasonable time.
+    Note it is not only the usual correctness assumptions but also frame conditions)
+  * If we verify Cogent bits and verify C bits then the FFI tells us how to put everything together
+    so the entire system is verified
+    (FFI specified some interface which gets you from C all the way up to the shallow embedding
+     The interface we defined was never tested
+     What we did before?
+        Here is a Cogent program that uses a bunch of C. The FFI defines how to compose the Cogent and
+          the C to get an overall proof of correctness. Note however, that this FFI assumes that it
+          has access to a bunch of abstraction functions on types, values, representations, etc, that
+          relate C \<rightarrow> Update \<rightarrow> Value_m \<rightarrow> Value_p \<rightarrow> Shallow and that the abstraction functions respect
+          a bunch of assumptions..
+        Can we actually provide these and discharge the assumptions in order to instantiate the FFI?
+          - abs typing that satisfy locale assumptions
+          - abstractions for abstract values in the update, value and shallow semantics
+          - value relations between C and update, update and value, and value and shallow
+          - abstractions for the abstract functions in the update, value and shallow semantics
+          - proofs for preservation in the update and value semantics for each abstract function
+          - proofs for mono renaming for each abstract function
+          - proofs for correspondence between C and update, update and value, and value and shallow
+          - proofs that the abstraction for the abstract functions in the value semantics execute
+            if the the abstraction for the corresponding abstract function in the update semantics
+            executes
+
+
+
+  * Verified library for word arrays
+      * BilbyFS, Ext2FS
+*)
+thm corres_def corres_app_concrete corres_app_abstract
+thm wordarray_fold_no_break_0'_def[simplified] hoare_add_K dispatch_t4'_def
+
+abbreviation "mk_urecord xs \<equiv> URecord (map (\<lambda>x. (x, upd.uval_repr x)) xs)"
+definition "foldmap_measure i end \<equiv> unat end - unat i"
+definition "foldmap_bounds frm to len i e 
+  \<equiv> frm \<le> i \<and> e = min to len \<and> (frm < e \<longrightarrow> i < e) \<and> (\<not>(frm < e) \<longrightarrow> frm = i)"
+definition "foldmap_inv foldmap \<xi>' \<sigma> s' p frm i f acc obsv r res'
+  \<equiv> (\<exists>\<sigma>' res. foldmap \<xi>' \<sigma> p frm i f acc obsv r (\<sigma>', res) \<and> val_rel res res' \<and> (\<sigma>', s') \<in> state_rel)"
+lemma state_rel_ex: 
+  "\<exists>\<sigma>. (\<sigma>, s) \<in> state_rel"
+  apply (clarsimp simp: state_rel_def heap_rel_def heap_rel_ptr_def heap_rel_ptr_w32_def)
+  apply (rule_tac x = "\<lambda>_. option.None" in exI)
+  apply clarsimp
+  done
+
+lemma whileLoop_add_invI:
+  assumes "\<lbrace> P \<rbrace> whileLoop_inv c b init I (measure M) \<lbrace> Q \<rbrace>!"
+  shows "\<lbrace> P \<rbrace> whileLoop c b init \<lbrace> Q \<rbrace>!"
+  by (metis assms whileLoop_inv_def)
+
+lemma
+  "cogent_function_val_rel f (sint FUN_ENUM_mul) \<Longrightarrow> 
+    \<forall>x x' \<sigma> s. val_rel x x' \<longrightarrow> update_sem_init.corres wa_abs_typing_u wa_abs_repr (Generated.state_rel wa_abs_repr) 
+      (App (uvalfun_to_exprfun f) (Var 0)) (do ret <- dispatch_t4' FUN_ENUM_mul x'; gets (\<lambda>s. ret) od) 
+      \<xi>_0 [x] \<Xi> [option.Some (foldmap_funarg_type ''wordarray_fold_no_break_0'')] \<sigma> s"
+  apply (clarsimp simp: cogent_function_val_rel untyped_func_enum_defs)
+  apply (rule corres_app_concrete[simplified]; simp?)
+  apply (subgoal_tac "foldmap_funarg_type ''wordarray_fold_no_break_0'' = prod.fst (prod.snd Generated_TypeProof.mul_type)")
+   apply (monad_eq simp: dispatch_t4'_def FUN_ENUM_mul_def unknown_bind_ignore \<Xi>_def)
+   apply (rule corres_mul; simp)
+  apply (clarsimp simp: \<Xi>_def wordarray_fold_no_break_0_type_def mul_type_def abbreviated_type_defs)
+  done
+thm validNF_def valid_def no_fail_def
+
+lemma fold_dispatch_wp:
+  "\<lbrakk>wa_abs_typing_u (UWA (TPrim (Num t)) len arr) ''WordArray'' [TPrim (Num t)] s r w \<sigma>;
+    (\<Xi>, [], [option.Some (foldmap_funarg_type ''wordarray_fold_no_break_0'')] \<turnstile> 
+    (App f (Var 0)) : (foldmap_funret_type ''wordarray_fold_no_break_0''));
+    \<forall>x x' \<sigma> s. val_rel x x' \<longrightarrow>
+      update_sem_init.corres wa_abs_typing_u wa_abs_repr (Generated.state_rel wa_abs_repr) 
+        (App f (Var 0)) (do ret <- dispatch_t4' f_num x'; gets (\<lambda>s. ret) od) 
+        \<xi>0 [x] \<Xi> [option.Some (foldmap_funarg_type ''wordarray_fold_no_break_0'')] \<sigma> s\<rbrakk> \<Longrightarrow>
+    \<lbrace>\<lambda>sa. (a', n') = (a, n) \<and> (\<exists>x v. args = t3_C.elem_C_update (\<lambda>_. v) a \<and>
+          \<sigma> (arr + size_of_num_type t * n) = option.Some x \<and> val_rel x v) \<and>
+      foldmap_inv upd_wa_foldnb_bod \<xi>0 \<sigma> sa p frm n f acc obsv r_set (t3_C.acc_C args) \<and>
+      foldmap_bounds frm to len n e\<rbrace>
+      dispatch_t4' f_num args 
+    \<lbrace>\<lambda>ret sb. foldmap_inv upd_wa_foldnb_bod \<xi>0 \<sigma> sb p frm (n + 1) f acc obsv r_set ret \<and>
+      foldmap_bounds frm to len (n + 1) e \<and>
+      foldmap_measure (n + 1) to < foldmap_measure n' to\<rbrace>!"
+  sorry
+thm corres_sum
+lemma upd_C_wordarray_fold_no_break_corres':
+  "\<lbrakk>i < length \<gamma>; val_rel (\<gamma> ! i) v'; \<Gamma>' ! i = option.Some (prod.fst (prod.snd (\<Xi> ''wordarray_fold_no_break_0'')));
+   \<gamma> ! i = URecord fs; f = prod.fst (fs ! 3); upd.proc_env_matches_ptrs \<xi>0 \<Xi>;
+  (\<Xi>, [], [option.Some (foldmap_funarg_type ''wordarray_fold_no_break_0'')] \<turnstile> 
+    (App (uvalfun_to_exprfun f) (Var 0)) : (foldmap_funret_type ''wordarray_fold_no_break_0''));
+   \<forall>x x' \<sigma> s. val_rel x x' \<longrightarrow> update_sem_init.corres wa_abs_typing_u wa_abs_repr (Generated.state_rel wa_abs_repr) 
+      (App (uvalfun_to_exprfun f) (Var 0)) (do ret <- dispatch_t4' (t5_C.f_C v') x'; gets (\<lambda>s. ret) od) 
+      \<xi>0 [x] \<Xi> [option.Some (foldmap_funarg_type ''wordarray_fold_no_break_0'')] \<sigma> s\<rbrakk>
+    \<Longrightarrow> update_sem_init.corres wa_abs_typing_u wa_abs_repr (Generated.state_rel wa_abs_repr)
+         (App (AFun ''wordarray_fold_no_break_0'' []) (Var i)) (do x <- main_pp_inferred.wordarray_fold_no_break_0' v';
+gets (\<lambda>s. x)
+                                                                od)
+         \<xi>1 \<gamma> \<Xi>  \<Gamma>' \<sigma> s"
+  apply (rule absfun_corres; simp)
+  apply (clarsimp simp: abs_fun_rel_def'; rename_tac r w)
+  apply (thin_tac "\<Gamma>' ! i = _")
+  apply (subst \<xi>1.simps)
+  apply (subst (asm) val_rel_simp; clarsimp)
+  apply (subst (asm) val_rel_ptr_def; clarsimp)
+  apply (subst (asm) val_rel_fun_tag)
+  apply (subst (asm) val_rel_word)
+  apply (subst (asm) val_rel_word)
+  apply (clarsimp simp: upd_wa_foldnb_def wordarray_fold_no_break_0'_def)
+  apply (rename_tac pwa_rep frm_rep to_rep f_rep acc a_rep obsv o_rep wa_rep)
+  apply (erule upd.u_t_recE; clarsimp)
+  apply (rotate_tac -3)
+  apply (subst (asm) \<Xi>_def; clarsimp simp: wordarray_fold_no_break_0_type_def abbreviated_type_defs)
+  apply (erule upd.u_t_r_consE; clarsimp)
+  apply (erule upd.u_t_p_absE; clarsimp)
+  apply (frule wa_abs_typing_u_elims(1); clarsimp)
+  apply (erule upd.u_t_r_consE; simp)
+  apply (erule upd.u_t_r_consE; simp)
+  apply (erule conjE)+
+  apply (drule_tac t = "type_repr _" in sym)+
+  apply clarsimp
+  apply (erule upd.u_t_primE)+
+  apply (drule_tac t = "lit_type _" in sym)+
+  apply clarsimp
+  apply (erule upd.u_t_r_consE; clarsimp)+
+  apply (erule upd.u_t_r_emptyE; clarsimp)
+  apply (frule upd.tfun_no_pointers(1))
+  apply (frule upd.tfun_no_pointers(2))
+  apply clarsimp
+  apply (rename_tac acc ra wa obsv ro wo)
+  apply (subst unknown_bind_ignore)+
+  apply clarsimp
+  apply wp
+      apply (clarsimp simp: unknown_bind_ignore split: prod.split)
+      apply (rename_tac var e)
+      apply (rule_tac M = "\<lambda>((_, i), _). foldmap_measure i (t5_C.to_C v')" and 
+      I = "\<lambda>(a, b) s. foldmap_inv upd_wa_foldnb_bod \<xi>0 \<sigma> s (ptr_val (t5_C.arr_C v'))
+          (t5_C.frm_C v') b (uvalfun_to_exprfun f) acc obsv (ra \<union> ro) (t3_C.acc_C a) \<and> 
+        foldmap_bounds (t5_C.frm_C v') (t5_C.to_C v') len b e" in whileLoop_add_invI; simp?)
+      apply (wp; clarsimp simp: unknown_bind_ignore split: prod.splits)
+           apply (rename_tac sa a n args a' n')
+           apply (rule_tac a = a in fold_dispatch_wp; simp?)
+            apply (clarsimp simp: \<Xi>_def wordarray_fold_no_break_0_type_def abbreviated_type_defs)
+           apply (clarsimp simp: \<Xi>_def wordarray_fold_no_break_0_type_def abbreviated_type_defs)
+          apply wp
+         apply wp
+        apply wp
+       apply clarsimp
+
+  oops
+  thm cogent_function_val_rel
+  find_theorems name:"add_inv"
+(*
+abbreviation "wordarray_foldnb_inv \<xi>' \<sigma> p frm i f acc obsv t to v
+  \<equiv> (\<lambda>(a, b) s. (\<exists>\<sigma> r. upd_wa_foldnb_bod \<xi>' ))"
+*)
 end (* of context *)
 end
