cogent/examples/wa_connect/WordArray_CorresProof_Asm.thy
@@ -3,39 +3,12 @@
   word array functions.
 *)
 theory WordArray_CorresProof_Asm
-  imports WordArray_Abstractions
+  imports WordArray_UAbsFun WordArray_VAbsFun
 begin
 
 context WordArray begin
 
 section "Level 0 Assumptions"
-
-lemma val_wa_length_rename_monoexpr_correct:
-  "\<lbrakk>val_wa_length (val.rename_val rename' (val.monoval v)) v'; val.proc_env_matches \<xi>\<^sub>v \<Xi>'; proc_ctx_wellformed \<Xi>'\<rbrakk>
-    \<Longrightarrow> v' = val.rename_val rename' (val.monoval v') \<and> val_wa_length v v'"
-  apply (clarsimp simp: val_wa_length_def)
-  apply (case_tac v; clarsimp)
-  done
-
-lemma val_wa_get_rename_monoexpr_correct:
-  "\<lbrakk>val_wa_get (val.rename_val rename' (val.monoval v)) v'; val.proc_env_matches \<xi>\<^sub>v \<Xi>'; proc_ctx_wellformed \<Xi>'\<rbrakk>
-    \<Longrightarrow> v' = val.rename_val rename' (val.monoval v') \<and> val_wa_get v v'"
-  apply (clarsimp simp: val_wa_get_def)
-  apply (case_tac v; clarsimp)
-  apply (case_tac z; clarsimp)
-  apply (case_tac za; clarsimp)
-  done
-
-lemma val_wa_put2_rename_monoexpr_correct:
-  "\<lbrakk>val_wa_put2 (val.rename_val rename' (val.monoval v)) v'; val.proc_env_matches \<xi>\<^sub>v \<Xi>'; proc_ctx_wellformed \<Xi>'\<rbrakk>
-    \<Longrightarrow> v' = val.rename_val rename' (val.monoval v') \<and> val_wa_put2 v v'"
-  apply (clarsimp simp: val_wa_put2_def)
-  apply (case_tac v; clarsimp)
-  apply (case_tac z; clarsimp)
-  apply (case_tac za; clarsimp)
-  apply (case_tac zb; clarsimp)
-  done
-
 
 lemma value_sem_rename_mono_prog_rename_\<Xi>_\<xi>m_\<xi>p: 
   "value_sem.rename_mono_prog wa_abs_typing_v rename \<Xi> \<xi>m \<xi>p"
@@ -59,37 +32,6 @@ lemma value_sem_rename_mono_prog_rename_\<Xi>_\<xi>m_\<xi>p:
   apply (subst (asm) assoc_lookup.simps)+
   apply (clarsimp split: if_split_asm)
   apply (clarsimp simp: val_wa_put2_rename_monoexpr_correct)
-  done
-
-lemma val_wa_get_preservation:
-  "\<lbrakk>val.vval_typing \<Xi>' v (TRecord [(a, TCon ''WordArray'' [t] (Boxed ReadOnly ptrl), Present),
-      (b, TPrim (Num U32), Present)] Unboxed); val_wa_get v v'\<rbrakk>
-    \<Longrightarrow> val.vval_typing \<Xi>' v' t"
-  apply (clarsimp simp: val_wa_get_def)
-  apply (erule val.v_t_recordE; clarsimp)
-  apply (erule val.v_t_r_consE; clarsimp)+
-  apply (erule val.v_t_abstractE; clarsimp simp: wa_abs_typing_v_def)
-  apply (rule val.v_t_prim'; clarsimp)
-  done
-
-lemma val_wa_length_preservation:
-  "\<lbrakk>val.vval_typing \<Xi>' v (TCon ''WordArray'' [t] (Boxed ReadOnly ptrl)); val_wa_length v v'\<rbrakk>
-    \<Longrightarrow> val.vval_typing \<Xi>' v' (TPrim (Num U32))"
-  apply (clarsimp simp:  val_wa_length_def)
-  apply (rule val.v_t_prim'; clarsimp)
-  done
-
-lemma val_wa_put2_preservation:
-  "\<lbrakk>val.vval_typing \<Xi>' v (TRecord [(a, TCon ''WordArray'' [t] (Boxed Writable ptrl), Present),
-      (b', TPrim (Num U32), Present), (c, t, Present)] Unboxed); val_wa_put2 v v'\<rbrakk>
-    \<Longrightarrow> val.vval_typing \<Xi>' v' (TCon ''WordArray'' [t] (Boxed Writable ptrl))"
-  apply (clarsimp simp: val_wa_put2_def)
-  apply (erule val.v_t_recordE)
-  apply (erule val.v_t_r_consE; clarsimp)
-  apply (erule val.v_t_abstractE)
-  apply (rule val.v_t_abstract; clarsimp)
-  apply (clarsimp simp: wa_abs_typing_v_def)
-  apply (case_tac "i = unat idx"; clarsimp)
   done
 
 lemma val_proc_env_matches_\<xi>m_\<Xi>:
@@ -162,7 +104,7 @@ lemma wa_length_upd_val:
   apply (clarsimp simp: val_wa_length_def)
   done
 
-inductive_cases u_v_t_prim_tE : "upd_val_rel \<Xi>' \<sigma> u v (TPrim l) r w"
+
 
 lemma wa_put2_upd_val:
   "\<lbrakk>upd_val_rel \<Xi>' \<sigma> au av (TRecord [(a, TCon ''WordArray'' [t] (Boxed Writable ptrl), Present),
@@ -190,7 +132,7 @@ lemma wa_put2_upd_val:
   apply (subst (asm) lit_type.simps)+
   apply clarsimp
   apply (erule type_repr.elims[where y = " RPrim _", simplified]; clarsimp)
-  apply (erule u_v_t_prim_tE)
+  apply (erule u_v_t_primtE)
   apply (rule conjI)
    apply clarsimp
    apply (clarsimp simp: val_wa_put2_def)
@@ -236,7 +178,6 @@ lemma wa_put2_upd_val:
   apply (clarsimp simp: val_wa_put2_def)
   done
 
-
 lemma proc_env_u_v_matches_\<xi>0_\<xi>m_\<Xi>:
   "proc_env_u_v_matches \<xi>0 \<xi>m \<Xi>"
   apply (clarsimp simp: proc_env_u_v_matches_def)
@@ -249,86 +190,6 @@ lemma proc_env_u_v_matches_\<xi>0_\<xi>m_\<Xi>:
    apply (drule wa_length_upd_val; simp)
   apply (clarsimp simp: wordarray_put2_0_type_def abbreviated_type_defs)
   apply (drule wa_put2_upd_val; simp)
-  done
-
-lemma upd_wa_get_preservation:
-  "\<lbrakk>upd.uval_typing \<Xi>' \<sigma> v (TRecord [(a, TCon ''WordArray'' [t] (Boxed ReadOnly ptrl), Present),
-      (b, TPrim (Num U32), Present)] Unboxed) r w; upd_wa_get_0 (\<sigma>, v) (\<sigma>', v')\<rbrakk>
-    \<Longrightarrow> \<exists>r' w'. upd.uval_typing \<Xi>' \<sigma>' v' t r' w' \<and> r' \<subseteq> r \<and> frame \<sigma> w \<sigma>' w'"
- apply (clarsimp simp:  upd_wa_get_0_def)
-  apply (erule upd.u_t_recE; clarsimp)
-  apply (erule upd.u_t_r_consE; clarsimp)
-  apply (erule upd.u_t_p_absE[where s = "Boxed ReadOnly _", simplified])
-  apply (drule_tac t = "type_repr _" in sym)+
-  apply clarsimp
-  apply (erule upd.u_t_r_consE; simp)
-  apply (erule conjE)+
-  apply (drule_tac t = "type_repr _" in sym)+
-  apply (erule upd.u_t_r_emptyE; clarsimp)
-  apply (erule upd.u_t_primE; subst (asm) lit_type.simps; clarsimp)+
-  apply (rule_tac x = "{}" in exI)+
-  apply (clarsimp simp: frame_def wa_abs_typing_u_def)
-  apply (erule_tac x = idx in allE)
-  apply (case_tac "idx < len"; clarsimp)
-   apply (rule upd.u_t_prim'; clarsimp)+
-  apply (case_tac ta; clarsimp intro!: upd.u_t_prim')
-  done
-
-lemma upd_wa_length_preservation:
-  "\<lbrakk>upd.uval_typing \<Xi>' \<sigma> v (TCon ''WordArray'' [t] (Boxed ReadOnly ptrl)) r w;
-    upd_wa_length_0 (\<sigma>, v) (\<sigma>', v')\<rbrakk>
-    \<Longrightarrow> \<exists>r' w'. upd.uval_typing \<Xi>' \<sigma>' v' (TPrim (Num U32)) r' w' \<and> r' \<subseteq> r \<and> frame \<sigma> w \<sigma>' w'"
-  apply (clarsimp simp: upd_wa_length_0_def)
-  apply (erule upd.u_t_p_absE; clarsimp)
-  apply (rule_tac x = "{}" in exI)+
-  apply (clarsimp simp: frame_def intro!: upd.u_t_prim')
-  done
-
-inductive_cases upd_u_t_prim_tE: "upd.uval_typing \<Xi>' \<sigma> u (TPrim l) r w"
-
-lemma upd_wa_put2_preservation:
-  "\<lbrakk>upd.uval_typing \<Xi>' \<sigma> v (TRecord [(a, TCon ''WordArray'' [t] (Boxed Writable ptrl), Present),
-      (b, TPrim (Num U32), Present), (c, t, Present)] Unboxed) r w; upd_wa_put2_0 (\<sigma>, v) (\<sigma>', v')\<rbrakk>
-    \<Longrightarrow> \<exists>r' w'. upd.uval_typing \<Xi>' \<sigma>' v' (TCon ''WordArray'' [t] (Boxed Writable ptrl)) r' w' \<and>
-      r' \<subseteq> r \<and> frame \<sigma> w \<sigma>' w'"
-  apply (clarsimp simp: upd_wa_put2_0_def)
-  apply (erule upd.u_t_recE; clarsimp)
-  apply (erule upd.u_t_r_consE; clarsimp)
-  apply (erule upd.u_t_p_absE[where s = "Boxed Writable _", simplified])
-  apply (drule_tac t = "type_repr _" in sym)+
-  apply clarsimp
-  apply (erule upd.u_t_r_consE; simp)
-  apply (erule conjE)+
-  apply (subst (asm) type_repr.simps[symmetric])+
-  apply clarsimp
-  apply (erule upd.u_t_r_consE; simp)
-  apply (erule conjE)+
-  apply (subst (asm) type_repr.simps[symmetric])+
-  apply clarsimp
-  apply (erule upd.u_t_r_emptyE)
-  apply (erule upd.u_t_primE)+
-  apply (subst (asm) lit_type.simps)+
-  apply clarsimp
-  apply (drule_tac t = "type_repr _" in sym)+
-  apply (erule type_repr.elims[where y = "RPrim _", simplified]; clarsimp)
-  apply (erule upd_u_t_prim_tE; clarsimp)
-  apply (rule_tac x = r in exI)
-  apply (rule_tac x = "insert p wa" in exI)
-  apply (rule conjI)
-  apply (drule_tac t = "lit_type _" in sym; clarsimp)
-   apply (rule_tac ptrl = ptrl and a = "UWA (TPrim (Num ta)) len arr" 
-      in upd.u_t_p_abs_w[where ts = "[TPrim _]", simplified]; simp?)
-    apply (clarsimp simp: wa_abs_typing_u_def split: prim_type.splits if_splits)
-   apply (frule wa_abs_typing_u_elims(3); clarsimp split: if_splits)
-  apply (clarsimp split: if_splits simp: upd.frame_id)
-  apply (drule_tac t = "lit_type _" in sym; clarsimp)
-  apply (frule wa_abs_typing_u_elims(3); clarsimp)
-  apply (clarsimp simp: frame_def)
-  apply (rule conjI; clarsimp)
-   apply (rule conjI, clarsimp)
-    apply (erule_tac x = idx in allE; clarsimp)+
-   apply (rule conjI; clarsimp)
-  apply (rule conjI; clarsimp)
   done
 
 lemma upd_proc_env_matches_ptrs_\<xi>0_\<Xi>:
@@ -364,301 +225,13 @@ lemma proc_ctx_wellformed_\<Xi>:
 
 section "Level 1 Assumptions"
 
-lemma upd_wa_foldnb_bod_preservation:
-  "\<lbrakk>proc_ctx_wellformed \<Xi>'; upd.proc_env_matches_ptrs \<xi>\<^sub>u \<Xi>';
-    upd_wa_foldnb_bod \<xi>\<^sub>u \<sigma> p frm to f acc obsv (rb \<union> rc) (\<sigma>', res);
-    \<sigma> p = option.Some (UAbstract (UWA t len arr)); 
-    wa_abs_typing_u (UWA t len arr) ''WordArray'' [t] (Boxed ReadOnly ptrl) ra wa \<sigma>;
-    upd.uval_typing \<Xi>' \<sigma> acc u rb wb; upd.uval_typing \<Xi>' \<sigma> obsv v rc {};  wb \<inter> rc = {};
-    \<Xi>', [], [option.Some (TRecord [
-      (b0, t, Present), (b1, u, Present), (b2, v, Present)] Unboxed)] \<turnstile> (App f (Var 0)) : u;
-    distinct [b0, b1, b2]\<rbrakk>
-    \<Longrightarrow> \<exists>r' w'. upd.uval_typing \<Xi>' \<sigma>' res u r' w' \<and> r' \<subseteq> ({p} \<union> ra \<union> rb \<union> rc) \<and> frame \<sigma> wb \<sigma>' w'"
-  apply (induct to arbitrary: \<sigma>' res)
-   apply (erule upd_wa_foldnb_bod.elims; clarsimp)
-   apply (rule_tac x = rb in exI)
-   apply (rule_tac x = wb in exI)
-   apply (clarsimp simp: upd.frame_id)
-  apply (case_tac "len < 1 + to")
-   apply (drule upd_wa_foldnb_bod_back_step'; simp?)
-  apply (case_tac "1 + to \<le> frm")
-   apply (frule_tac y = "1 + to" and x = frm in leD)
-   apply (erule upd_wa_foldnb_bod.elims; clarsimp)
-   apply (rule_tac x = rb in exI)
-   apply (rule_tac x = wb in exI)
-   apply (clarsimp simp: upd.frame_id)
-  apply (frule wa_abs_typing_u_elims(1); clarsimp)
-  apply (drule upd_wa_foldnb_bod_back_step; simp?)
-  apply clarsimp
-  apply (drule_tac x = \<sigma>'' in meta_spec)
-  apply (drule_tac x = r'' in meta_spec)
-  apply clarsimp
-  apply (frule wa_abs_typing_u_elims(5))
-  apply (erule_tac x = to in allE; clarsimp)+
-  apply (erule impE)
-   apply (cut_tac x = to in word_overflow)
-   apply (erule disjE; clarsimp simp: add.commute)
-   apply auto[1]
-  apply clarsimp
-  apply (drule_tac ?\<Gamma> = "[option.Some (TRecord [(b0, TPrim (Num ta), Present), (b1, u, Present),
-    (b2, v, Present)] Unboxed)]" and r = "r' \<union> rc" and  w = w' and \<tau> = u in upd.preservation_mono(1); simp?)
-   apply (rule upd.matches_ptrs_some[where ts = "[]" and r' = "{}" and w' = "{}", simplified])
-    apply (rule upd.u_t_struct; simp?)
-    apply (rule upd.u_t_r_cons1[where r = "{}" and w = "{}", simplified])
-      apply (rule upd.u_t_prim'; clarsimp)
-     apply (rule upd.u_t_r_cons1[where r' = rc and w' = "{}", simplified]; simp?)
-       apply (rule upd.u_t_r_cons1[where r' = "{}" and w' = "{}", simplified]; simp?)
-         apply (rule upd.uval_typing_frame(1); simp?)
-         apply blast
-        apply (rule upd.u_t_r_empty)
-       apply (drule_tac v = obsv in upd.type_repr_uval_repr(1); simp)
-      apply (rule disjointI)
-      apply (thin_tac "frame _ _ _ _")
-      apply (clarsimp simp: frame_def)
-      apply (erule_tac x = y in allE; clarsimp)+
-      apply (drule_tac x = y in orthD2; simp)
-      apply (drule_tac u = obsv and p = y in upd.uval_typing_valid(1)[rotated 1]; simp)
-     apply (drule_tac v = r'' in upd.type_repr_uval_repr(1); simp)
-    apply clarsimp
-   apply (rule upd.matches_ptrs_empty[where \<tau>s = "[]", simplified])
-  apply clarsimp
-  apply (thin_tac "frame _ _ _ _")
-  apply (rule_tac x = r'a in exI)
-  apply (rule_tac x = w'a in exI)
-  apply clarsimp
-  apply (rule conjI, blast)
-  apply (rule upd.frame_trans; simp)
-  done
-
-lemma readonly_not_in_frame:
-  "\<lbrakk>frame \<sigma> w \<sigma>' w'; \<sigma> p = option.Some v; p \<notin> w\<rbrakk> \<Longrightarrow> p \<notin> w'"
-  apply (frule_tac p = p in valid_ptr_not_in_frame_same; simp?)
-  by (clarsimp simp: frame_def)
-
-lemma frame_expand:
-  "\<lbrakk>frame \<sigma> w \<sigma>' w'; \<sigma> p \<noteq> option.None\<rbrakk> \<Longrightarrow> frame \<sigma> (insert p w) \<sigma>' (insert p w')"
-  "\<lbrakk>frame \<sigma> w \<sigma>' w'; \<forall>p\<in>s. \<sigma> p \<noteq> option.None\<rbrakk> \<Longrightarrow> frame \<sigma> (s \<union> w) \<sigma>' (s \<union> w')"
-   apply (clarsimp simp: frame_def)
-   apply (rule conjI; clarsimp)
-  apply (clarsimp simp: frame_def)
-  apply (rule conjI; clarsimp)
-  done
-
-lemma upd_wa_mapAccumnb_bod_preservation:
-  "\<lbrakk>proc_ctx_wellformed \<Xi>'; upd.proc_env_matches_ptrs \<xi>\<^sub>u \<Xi>'; (wa \<union> wb) \<inter> rc = {}; 
-    wa \<inter> wb = {}; wa \<inter> rb = {}; p \<notin> wa \<union> rb \<union> wb \<union> rc; \<sigma> p = option.Some (UAbstract (UWA t len arr));
-    upd_wa_mapAccumnb_bod \<xi>\<^sub>u \<sigma> p frm to f acc obsv (rb \<union> rc) (\<sigma>', res); 
-    wa_abs_typing_u (UWA t len arr) ''WordArray'' [t] (Boxed Writable ptrl) ra wa \<sigma>;
-    upd.uval_typing \<Xi>' \<sigma> acc u rb wb; upd.uval_typing \<Xi>' \<sigma> obsv v rc {};
-    \<Xi>', [], [option.Some (TRecord [(a0, t, Present), (a1, u, Present), (a2, v, Present)] Unboxed)] 
-      \<turnstile> (App f (Var 0)) : TRecord [(b0, t, Present), (b1, u, Present)] Unboxed;
-    distinct [a0, a1, a2]; distinct [b0, b1]\<rbrakk>
-    \<Longrightarrow> \<exists>r' w'. 
-      upd.uval_typing \<Xi>' \<sigma>' res (TRecord [(b0, (TCon ''WordArray'' [t] (Boxed Writable ptrl), Present)),
-        (b1, (u, Present))] Unboxed) r' (insert p w') \<and> 
-      r' \<subseteq> (ra \<union> rb \<union> rc) \<and> frame \<sigma> (wa \<union> wb) \<sigma>' w'"
-  apply (induct to arbitrary: \<sigma>' res)
-   apply (erule upd_wa_mapAccumnb_bod.elims; clarsimp)
-   apply (rule_tac x = "ra \<union> rb" in exI)
-   apply (rule_tac x = "wa \<union> wb" in exI)
-   apply (clarsimp simp: upd.frame_id)
-   apply (rule upd.u_t_struct; simp?)
-   apply (subst Set.Un_insert_left[symmetric])
-   apply (rule upd.u_t_r_cons1[where r' = rb and w' = wb, simplified]; simp?)
-     apply (rule_tac ptrl = ptrl and
-      a = "UWA (TPrim (Num ta)) len arr"
-      in upd.u_t_p_abs_w[where ts = "[TPrim _]", simplified]; simp?)
-     apply (drule_tac wa_abs_typing_u_elims(3); simp)
-    apply (rule upd.u_t_r_cons1[where r' = "{}" and w' = "{}", simplified]; simp?)
-     apply (rule upd.u_t_r_empty)
-    apply (drule upd.type_repr_uval_repr(1); simp)
-   apply (drule_tac wa_abs_typing_u_elims(3); simp)
-  apply (case_tac "len < 1 + to")
-   apply (drule upd_wa_mapAccumnb_bod_back_step'; simp?)
-  apply (case_tac "1 + to \<le> frm")
-   apply (frule_tac y = "1 + to" and x = frm in leD)
-   apply (erule upd_wa_mapAccumnb_bod.elims; clarsimp)
-   apply (rule_tac x = "ra \<union> rb" in exI)
-   apply (rule_tac x = "wa \<union> wb" in exI)
-   apply (clarsimp simp: upd.frame_id)
-   apply (rule upd.u_t_struct; simp?)
-   apply (subst Set.Un_insert_left[symmetric])
-   apply (rule upd.u_t_r_cons1[where r' = rb and w' = wb, simplified]; simp?)
-     apply (rule_tac ptrl = ptrl and
-      a = "UWA (TPrim (Num ta)) len arr"
-      in upd.u_t_p_abs_w[where ts = "[TPrim _]", simplified]; simp?)
-     apply (drule_tac wa_abs_typing_u_elims(3); simp)
-    apply (rule upd.u_t_r_cons1[where r' = "{}" and w' = "{}", simplified]; simp?)
-     apply (rule upd.u_t_r_empty)
-    apply (drule upd.type_repr_uval_repr(1); simp)
-   apply (drule_tac wa_abs_typing_u_elims(3); simp)
-  apply (subgoal_tac "to < len")
-   apply (frule_tac wa_abs_typing_u_elims(1); clarsimp)
-   apply (frule upd_wa_mapAccumnb_bod_preservation'; simp?)
-   apply clarsimp
-   apply (drule upd_wa_mapAccumnb_bod_back_step; simp?)
-    apply (drule wa_abs_typing_u_elims(6); simp)
-   apply clarsimp
-   apply (drule_tac x = \<sigma>'' in meta_spec)
-   apply (drule_tac x = "URecord [
-    (UPtr p (RCon ''WordArray'' [RPrim (Num ta)]), RPtr (RCon ''WordArray'' [RPrim (Num ta)])),
-    (r'', upd.uval_repr r'')]" in meta_spec)
-   apply clarsimp
-   apply (erule upd.u_t_recE; clarsimp)
-   apply (erule upd.u_t_r_consE; simp?)
-  apply (erule conjE)+
-   apply (drule_tac t = "type_repr _" in sym)+
-   apply clarsimp
-   apply (erule upd.u_t_r_consE; simp?)
-  apply (erule conjE)+
-   apply (drule_tac t = "type_repr _" in sym)+
-   apply clarsimp
-   apply (erule upd.u_t_r_emptyE; clarsimp)
-   apply (drule_tac r = "raa \<union> rc" and 
-      w = waa and
-      ?\<Gamma> = "[option.Some (TRecord [(a0, TPrim (Num ta), Present), (a1, u, Present), (a2, v, Present)] Unboxed)]" and
-      \<tau> = "TRecord [(b0, TPrim (Num ta), Present), (b1, u, Present)] Unboxed" 
-      in upd.preservation_mono(1); simp?)
-    apply (rule upd.matches_ptrs_some[where ts = "[]" and r' = "{}" and w' = "{}", simplified])
-     apply (rule upd.u_t_struct; simp?)
-     apply (rule upd.u_t_r_cons1[where r = "{}" and w = "{}", simplified])
-       apply (drule wa_abs_typing_u_elims(5))
-       apply (erule_tac x = to in allE)
-       apply clarsimp
-       apply (rule upd.u_t_prim'; clarsimp)
-      apply (rule upd.u_t_r_cons1[where r' = rc and w' = "{}", simplified]; simp?)
-       apply (rule upd.u_t_r_cons1[where r' = "{}" and w' = "{}", simplified]; simp?)
-         apply (rule upd.uval_typing_frame(1); simp?)
-         apply blast
-        apply (rule upd.u_t_r_empty)
-       apply (drule_tac v = obsv in upd.type_repr_uval_repr(1); simp)
-      apply (rule disjointI)
-      apply (frule_tac p = y and u = obsv in upd.uval_typing_valid(1)[rotated 1]; simp)
-      apply clarsimp
-      apply (drule_tac x = y in orthD2; simp)
-      apply clarsimp
-      apply (drule_tac p = y and  \<sigma> = \<sigma> in readonly_not_in_frame; simp?)
-      apply (subgoal_tac "y \<notin> w \<union> waa")
-       apply blast
-      apply (drule_tac t = "w \<union> waa" in sym)
-      apply simp
-      apply blast
-     apply (frule wa_abs_typing_u_elims(5))
-     apply (erule_tac x = to in allE)
-     apply clarsimp
-    apply (rule upd.matches_ptrs_empty[where \<tau>s = "[]", simplified])
-   apply clarsimp
-   apply (thin_tac "frame _ _ _ _")
-   apply (cut_tac v = v' and l = "arr + size_of_num_type ta * to" and \<sigma> = \<sigma>''' in frame_single_update)
-   apply (rule_tac x = r' in exI)
-   apply (rule_tac x = "{arr + size_of_num_type ta * i |i. i < len} \<union> w'a" in exI)
-   apply clarsimp
-   apply (erule upd.u_t_recE; clarsimp)
-   apply (erule upd.u_t_r_consE; simp?)
-   apply (erule conjE)+
-   apply (drule_tac t = "type_repr _" in sym)+
-   apply clarsimp
-   apply (erule upd.u_t_r_consE; simp?)
-   apply (erule conjE)+
-   apply clarsimp
-   apply (erule upd.u_t_r_emptyE; clarsimp)
-   apply (erule upd_u_t_prim_tE; clarsimp)
-   apply (erule upd.u_t_p_absE[where s = "Boxed Writable _", simplified])
-   apply (drule_tac s = "RCon _ _" in sym)
-   apply (drule_tac t = "lit_type _" in sym; clarsimp)
-   apply (frule_tac p = p and \<sigma> = \<sigma> in valid_ptr_not_in_frame_same; simp?)
-   apply clarsimp
-   apply (rule conjI)
-    apply (rule upd.u_t_struct; simp?)
-    apply (rule_tac upd.u_t_r_cons1[where r = "{}" and w = "insert _ _", simplified]; simp?)
-       apply (rule_tac ptrl = ptrl and
-      a = "UWA (TPrim (Num ta)) len arr"
-      in upd.u_t_p_abs_w[where ts = "[TPrim _]", simplified]; simp?)
-         apply (frule_tac \<sigma> = \<sigma>'' in wa_abs_typing_u_elims(3); clarsimp)
-         apply (drule_tac \<sigma> = \<sigma>'' and \<sigma>' = \<sigma>''' in upd.abs_typing_frame; simp?)
-         apply (rule wa_abs_typing_u_update; simp?)
-        apply (rule conjI; clarsimp)
-         apply (frule wa_abs_typing_u_elims(5))
-         apply (erule_tac x = to in allE)
-         apply clarsimp
-        apply (drule_tac p = p and \<sigma> = \<sigma>'' in valid_ptr_not_in_frame_same; simp?)
-       apply (drule wa_abs_typing_u_elims(3); clarsimp)
-      apply (rule upd.u_t_r_cons1[where r' = "{}" and w' = "{}", simplified]; simp?)
-       apply (drule_tac u = xb and r = rca and w = wc and \<sigma> = \<sigma>''' in upd.uval_typing_frame(1); simp?)
-        apply (frule_tac p = "arr + size_of_num_type ta * to" in upd.abs_typing_valid; simp?)
-         apply (drule wa_abs_typing_u_elims(3); clarsimp)
-         apply (rule_tac x = to in exI; simp)
-        apply clarsimp
-        apply (frule_tac w = wba in wa_abs_typing_u_elims(5))
-        apply (erule_tac x = to in allE; clarsimp)
-        apply (drule_tac p = "arr + size_of_num_type ta * to" and \<sigma> = \<sigma>'' in readonly_not_in_frame; simp?)
-        apply (drule_tac x = "arr + size_of_num_type ta * to" and S = wba in orthD1; simp?)
-        apply (drule_tac w = wba in wa_abs_typing_u_elims(3); clarsimp)
-        apply (rule_tac x = to in exI; simp)
-       apply (drule_tac x = "arr + size_of_num_type ta * to" and S = wba and S' = raa in orthD1; simp?)
-        apply (drule_tac w = wba in wa_abs_typing_u_elims(3); clarsimp)
-        apply (rule_tac x = to in exI; simp)
-       apply (drule_tac x = "arr + size_of_num_type ta * to" and S' = rc in orthD1; simp?)
-        apply (rule disjI1)
-        apply (drule wa_abs_typing_u_elims(3); clarsimp)
-        apply (rule_tac x = to in exI; clarsimp)
-       apply clarsimp
-       apply (drule_tac A = rca and B = "raa \<union> rc" and x = "arr + size_of_num_type ta * to" in in_mono)
-       apply blast
-      apply (rule upd.u_t_r_empty)
-     apply (frule_tac p = p  and \<sigma> = \<sigma>'' in readonly_not_in_frame; simp?)
-     apply (rule disjointI)
-     apply (frule_tac p = "xa" in upd.abs_typing_valid; simp?)
-      apply clarsimp
-      apply (drule wa_abs_typing_u_elims(3); clarsimp)
-     apply clarsimp
-     apply (frule_tac \<sigma> = \<sigma>'' in wa_abs_typing_u_elims(5))
-     apply (erule_tac x = i in allE; clarsimp)
-     apply (drule_tac p = "arr + size_of_num_type ta * i" and \<sigma> = \<sigma>'' in readonly_not_in_frame; simp?)
-     apply (drule_tac x = "arr + size_of_num_type ta * i" and S = wba in orthD1; simp?)
-     apply (drule_tac w = wba in wa_abs_typing_u_elims(3); clarsimp)
-     apply (rule_tac x = i in exI; simp)
-    apply (rule conjI)
-     apply (drule_tac A = rca and B = "raa \<union> rc" and x = p in in_mono; clarsimp)
-    apply (rule disjointI)
-    apply (drule_tac A = rca and B = "raa \<union> rc" and x = xa in in_mono; clarsimp)
-    apply (erule disjE)
-     apply (drule_tac x = "arr + size_of_num_type ta * i" and S' = raa in orthD1; simp?)
-     apply (drule_tac w = wba in wa_abs_typing_u_elims(3); clarsimp)
-     apply (rule_tac x = i in exI; simp)
-    apply (drule_tac x = "arr + size_of_num_type ta * i" and S' = rc in orthD1; simp?)
-    apply (drule wa_abs_typing_u_elims(3); clarsimp)
-    apply (rule_tac x = i in exI; simp)
-   apply (rule conjI)
-    apply (drule_tac A = rca and B = "raa \<union> rc" and C = "ra \<union> rb \<union> rc" in subset_trans; simp?)
-   apply (frule_tac p = p  and \<sigma> = \<sigma> in readonly_not_in_frame; simp?)
-   apply (frule_tac A = "w'" and x = p and B = "wba \<union> waa" in insert_ident; simp?)
-   apply (drule_tac \<sigma> = \<sigma>'' and s = wba in frame_expand(2))
-    apply (frule_tac w = wba in wa_abs_typing_u_elims(5); clarsimp)
-    apply (drule_tac w = wba in wa_abs_typing_u_elims(3); clarsimp)
-    apply (thin_tac "\<forall>i. p = arr + size_of_num_type ta * i \<longrightarrow> \<not> i < len")
-    apply (erule_tac x = i in allE; clarsimp)
-   apply (drule_tac \<sigma> = \<sigma> and \<sigma>' = \<sigma>'' and \<sigma>'' = \<sigma>''' in upd.frame_trans; simp?)
-   apply (drule_tac \<sigma> = \<sigma> in upd.frame_app; simp?)
-   apply clarsimp
-   apply (subst (asm) insert_absorb[where A = "_ \<union> wb"])
-    apply clarsimp
-    apply (drule wa_abs_typing_u_elims(3); clarsimp)
-    apply (rule_tac x = to in exI; simp)
-   apply (subst (asm) insert_absorb[where A = "_ \<union> _"])
-    apply (drule_tac w = wba in wa_abs_typing_u_elims(3); clarsimp)
-    apply (rule_tac x = to in exI; simp)
-   apply (drule_tac w = wba in wa_abs_typing_u_elims(3); clarsimp)
-  apply (drule unatSuc; clarsimp simp: word_less_nat_alt word_le_nat_alt)
-  done
-
-lemma upd_wa_foldnb_0_preservation:
+lemma upd_wa_foldnb_preservation:
   "\<And>K a b \<sigma> \<sigma>' \<tau>s v v' r w.
    \<lbrakk>list_all2 (kinding []) \<tau>s K; wordarray_fold_no_break_0_type = (K, a, b);
     upd.uval_typing \<Xi> \<sigma> v (instantiate \<tau>s a) r w;
-    upd_wa_foldnb_0 \<Xi> \<xi>0 (foldmap_funarg_type ''wordarray_fold_no_break_0'') (\<sigma>, v) (\<sigma>', v')\<rbrakk>
+    upd_wa_foldnb \<Xi> \<xi>0 (foldmap_funarg_type ''wordarray_fold_no_break_0'') (\<sigma>, v) (\<sigma>', v')\<rbrakk>
     \<Longrightarrow> \<exists>r' w'. upd.uval_typing \<Xi> \<sigma>' v' (instantiate \<tau>s b) r' w' \<and> r' \<subseteq> r \<and> frame \<sigma> w \<sigma>' w'"
-  apply (clarsimp simp: wordarray_fold_no_break_0_type_def upd_wa_foldnb_0_def)
+  apply (clarsimp simp: wordarray_fold_no_break_0_type_def upd_wa_foldnb_def)
   apply (rename_tac rb wb rc)
   apply (erule upd.u_t_recE; clarsimp)
   apply (erule upd.u_t_r_consE; clarsimp)
@@ -688,8 +261,6 @@ lemma upd_wa_foldnb_0_preservation:
   apply (elim upd.u_t_functionE upd.u_t_afunE; clarsimp; blast)+
   done
 
-inductive_cases v_t_prim_tE : "val.vval_typing \<Xi>' v (TPrim l)"
-
 lemma lit_type_ex:
   "lit_type l = Bool \<Longrightarrow> \<exists>v. l = LBool v"
   "lit_type l = Num U8 \<Longrightarrow> \<exists>v. l = LU8 v"
@@ -698,171 +269,6 @@ lemma lit_type_ex:
   "lit_type l = Num U64 \<Longrightarrow> \<exists>v. l = LU64 v"
   apply (induct l; clarsimp)+
   done
-
-lemma val_wa_foldnb_bod_rename_monoexpr_correct:
-  "\<lbrakk>val.proc_env_matches \<xi>\<^sub>m \<Xi>'; proc_ctx_wellformed \<Xi>'; 
-    value_sem.rename_mono_prog wa_abs_typing_v rename' \<Xi>' \<xi>\<^sub>m \<xi>\<^sub>p;
-    val_wa_foldnb_bod \<xi>\<^sub>m t xs frm to (vvalfun_to_exprfun (val.rename_val rename' (val.monoval f))) 
-      (val.rename_val rename' (val.monoval acc )) (val.rename_val rename' (val.monoval obsv)) r;
-    is_vval_fun (val.rename_val rename' (val.monoval f)); wa_abs_typing_v (VWA t xs) ''WordArray'' [t]; 
-    val.vval_typing \<Xi>' (val.rename_val rename' (val.monoval acc )) u;
-    val.vval_typing \<Xi>' (val.rename_val rename' (val.monoval obsv)) v;
-    \<Xi>', [], [option.Some (TRecord [(a0, t, Present), (a1, u, Present), (a2, v, Present)] Unboxed)] \<turnstile>
-      App (vvalfun_to_exprfun (val.rename_val rename' (val.monoval f))) (Var 0) : u; 
-    distinct [a0, a1, a2]\<rbrakk>
-       \<Longrightarrow> is_vval_fun f \<and> (\<exists>r'. r = val.rename_val rename' (val.monoval r') \<and>
-         val_wa_foldnb_bod \<xi>\<^sub>p t xs frm to (vvalfun_to_exprfun f) acc obsv r')"
-  apply (rule conjI)
-   apply (case_tac f; clarsimp)
-  apply (induct to arbitrary: r)
-   apply (erule val_wa_foldnb_bod.elims; clarsimp)
-   apply (subst val_wa_foldnb_bod.simps; clarsimp)
-  apply (case_tac "length xs < Suc to")
-   apply (drule val_wa_foldnb_bod_back_step'; simp)
-   apply (drule val_wa_foldnb_bod_to_geq_lenD)
-    apply linarith
-   apply (drule_tac x = r in meta_spec)
-   apply clarsimp
-   apply (erule meta_impE)
-    apply (rule val_wa_foldnb_bod_to_geq_len; simp?)
-   apply clarsimp
-   apply (rule_tac x = r' in exI; clarsimp)
-   apply (rule val_wa_foldnb_bod_to_geq_len; simp?)
-   apply (drule_tac to = to in val_wa_foldnb_bod_to_geq_lenD; simp?)
-  apply (case_tac "frm \<ge> Suc to")
-   apply (clarsimp simp: not_less not_le)
-   apply (erule val_wa_foldnb_bod.elims; clarsimp)
-   apply (subst val_wa_foldnb_bod.simps; clarsimp)
-  apply (drule val_wa_foldnb_bod_back_step; simp?)
-  apply clarsimp
-  apply (drule_tac x = r' in meta_spec)
-  apply clarsimp
-  apply (frule_tac \<gamma> = "[VRecord [xs ! to, r'a, obsv]]" and
-      ?\<Gamma> = "[option.Some (TRecord [(a0, t, Present), (a1, u, Present), (a2, v, Present)] Unboxed)]" and
-      e = "App (vvalfun_to_exprfun f) (Var 0)" and
-      v' = r and
-      \<tau> = u in val.rename_monoexpr_correct(1); simp?)
-     apply (clarsimp simp: val.matches_Cons[where xs = "[]" and ys = "[]", simplified])
-     apply (clarsimp simp: val.matches_def)
-     apply (rule val.v_t_record; simp?)
-     apply (rule val.v_t_r_cons1; clarsimp?)
-      apply (frule wa_abs_typing_v_elims(1); clarsimp)
-      apply (drule wa_abs_typing_v_elims(2))
-      apply (erule_tac x = to in allE; clarsimp)
-      apply (rule val.v_t_prim'; clarsimp)
-     apply (rule val.v_t_r_cons1; clarsimp?)
-      apply (drule val_wa_foldnb_bod_preservation; simp?)
-     apply (rule val.v_t_r_cons1; clarsimp?)
-     apply (rule val.v_t_r_empty)
-    apply (frule wa_abs_typing_v_elims(1); clarsimp)
-    apply (drule wa_abs_typing_v_elims(2))
-    apply (erule_tac x = to in allE; clarsimp)
-    apply (case_tac f; clarsimp)
-   apply (case_tac f; clarsimp)
-  apply clarsimp
-  apply (drule_tac \<xi>\<^sub>v = \<xi>\<^sub>p in val_wa_foldnb_bod_step; simp?)
-  apply (rule_tac x = va in exI)
-  apply clarsimp
-  done
-
-lemma val_wa_mapAccumnb_bod_rename_monoexpr_correct:
-  "\<lbrakk>val.proc_env_matches \<xi>\<^sub>m \<Xi>'; proc_ctx_wellformed \<Xi>'; 
-    value_sem.rename_mono_prog wa_abs_typing_v rename' \<Xi>' \<xi>\<^sub>m \<xi>\<^sub>p;
-    val_wa_mapAccumnb_bod \<xi>\<^sub>m t xs frm to (vvalfun_to_exprfun (val.rename_val rename' (val.monoval f))) 
-      (val.rename_val rename' (val.monoval acc )) (val.rename_val rename' (val.monoval obsv)) r;
-    is_vval_fun (val.rename_val rename' (val.monoval f)); wa_abs_typing_v (VWA t xs) ''WordArray'' [t]; 
-    val.vval_typing \<Xi>' (val.rename_val rename' (val.monoval acc )) u;
-    val.vval_typing \<Xi>' (val.rename_val rename' (val.monoval obsv)) v;
-    \<Xi>', [], [option.Some (TRecord [(a0, t, Present), (a1, u, Present), (a2, v, Present)] Unboxed)] \<turnstile>
-      App (vvalfun_to_exprfun (val.rename_val rename' (val.monoval f))) (Var 0) :
-      TRecord [(b0, t, Present), (b1, u, Present)] Unboxed; distinct [a0, a1, a2]; distinct [b0, b1]\<rbrakk>
-       \<Longrightarrow> is_vval_fun f \<and> (\<exists>r'. r = val.rename_val rename' (val.monoval r') \<and>
-         val_wa_mapAccumnb_bod \<xi>\<^sub>p t xs frm to (vvalfun_to_exprfun f) acc obsv r')"
-  apply (rule conjI)
-   apply (case_tac f; clarsimp)
-  apply (induct to arbitrary: r)
-   apply (erule val_wa_mapAccumnb_bod.elims; clarsimp)
-   apply (subst val_wa_mapAccumnb_bod.simps; clarsimp)
-  apply (case_tac "length xs < Suc to")
-   apply (drule val_wa_mapAccumnb_bod_back_step'; simp)
-   apply (drule val_wa_mapAccumnb_bod_to_geq_lenD)
-    apply linarith
-   apply (drule_tac x = r in meta_spec)
-   apply clarsimp
-   apply (erule meta_impE)
-    apply (rule val_wa_mapAccumnb_bod_to_geq_len; simp?)
-   apply clarsimp
-   apply (rule_tac x = r' in exI; clarsimp)
-   apply (rule val_wa_mapAccumnb_bod_to_geq_len; simp?)
-   apply (drule_tac to = to in val_wa_mapAccumnb_bod_to_geq_lenD; simp?)
-  apply (case_tac "frm \<ge> Suc to")
-  apply (clarsimp simp: not_less not_le)
-   apply (erule val_wa_mapAccumnb_bod.elims; clarsimp)
-   apply (subst val_wa_mapAccumnb_bod.simps; clarsimp)
-  apply (frule val_wa_mapAccumnb_bod_preservation'; clarsimp)
-  apply (drule val_wa_mapAccumnb_bod_back_step; simp?)
-  apply clarsimp
-  apply (drule_tac x = "VRecord [VAbstract (VWA t (rxs[to := xs ! to])), racc']" in meta_spec)
-  apply clarsimp
-  apply (case_tac r'; clarsimp)
-  apply (case_tac z; clarsimp)
-  apply (frule_tac \<gamma> = "[VRecord [xs ! to, za, obsv]]" and
-      ?\<Gamma> = "[option.Some (TRecord [(a0, t, Present), (a1, u, Present), (a2, v, Present)] Unboxed)]" and
-      e = "App (vvalfun_to_exprfun f) (Var 0)" and
-      v' = "VRecord [rxs ! to, racc]" and
-      \<tau> = "TRecord [(b0, t, Present), (b1, u, Present)] Unboxed" 
-      in val.rename_monoexpr_correct(1); simp?)
-     apply (clarsimp simp: val.matches_Cons[where xs = "[]" and ys = "[]", simplified])
-     apply (clarsimp simp: val.matches_def)
-     apply (rule val.v_t_record; simp?)
-     apply (rule val.v_t_r_cons1; clarsimp?)
-      apply (frule wa_abs_typing_v_elims(1); clarsimp)
-      apply (drule wa_abs_typing_v_elims(2))
-      apply (erule_tac x = to in allE; clarsimp)
-      apply (rule val.v_t_prim'; clarsimp)
-     apply (rule val.v_t_r_cons1; clarsimp?)
-      apply (drule val_wa_mapAccumnb_bod_preservation; simp?)
-      apply (erule val.v_t_recordE; clarsimp)
-      apply (erule val.v_t_r_consE; clarsimp)+
-     apply (rule val.v_t_r_cons1; clarsimp?)
-     apply (rule val.v_t_r_empty)
-    apply (frule wa_abs_typing_v_elims(1); clarsimp)
-    apply (drule wa_abs_typing_v_elims(2))
-    apply (erule_tac x = to in allE; clarsimp)
-    apply (case_tac f; clarsimp)
-   apply (case_tac f; clarsimp)
-  apply clarsimp
-  apply (case_tac va; clarsimp)
-  apply (drule_tac \<xi>\<^sub>v = \<xi>\<^sub>p in val_wa_mapAccumnb_bod_step; simp?)
-  apply (rule_tac x = "VRecord [VAbstract (VWA t (rxs[to := z])), zb]" in exI)
-  apply clarsimp
-   apply (frule_tac e = "App (vvalfun_to_exprfun (val.rename_val rename' (val.monoval f))) (Var 0)" and
-      v = "VRecord [val.rename_val rename' (val.monoval z), val.rename_val rename' (val.monoval zb)]" and
-      \<gamma> = "[VRecord [xs ! to, val.rename_val rename' (val.monoval za), val.rename_val rename' (val.monoval obsv)]]" and
-      \<tau> = "TRecord [(b0, t, Present), (b1, u, Present)] Unboxed" and
-      \<Gamma> = "[option.Some (TRecord [(a0, t, Present), (a1, u, Present), (a2, v, Present)] Unboxed)]" 
-      in val.preservation(1)[of "[]" "[]" _ _ _  \<xi>\<^sub>m, simplified]; simp?)
-  apply (clarsimp simp: val.matches_def)
-  apply (rule val.v_t_record; simp?)
-   apply (rule val.v_t_r_cons1)
-    apply (frule wa_abs_typing_v_elims(1); clarsimp)
-    apply (drule wa_abs_typing_v_elims(2))
-    apply (erule_tac x = to in allE; clarsimp)
-    apply (rule val.v_t_prim'; clarsimp)
-   apply (rule val.v_t_r_cons1; simp?)
-    apply (drule val_wa_mapAccumnb_bod_preservation; simp?)
-    apply (erule val.v_t_recordE; clarsimp)
-    apply (erule val.v_t_r_consE; clarsimp)+
-   apply (rule val.v_t_r_cons1; simp?)
-   apply (rule val.v_t_r_empty)
-  apply (erule val.v_t_recordE; clarsimp)
-   apply (erule val.v_t_r_consE; clarsimp)+
-  apply (erule val.v_t_r_emptyE; simp)
-  apply (drule wa_abs_typing_v_elims(1); clarsimp)
-  apply (clarsimp simp: val.vval_typing.simps[of _ _ "TPrim _", simplified])
-  apply (case_tac z; clarsimp)
-  by (simp add: upd.list_helper)
-  
 
 lemma value_sem_rename_mono_prog_rename_\<Xi>_\<xi>m1_\<xi>p1: 
   "value_sem.rename_mono_prog wa_abs_typing_v rename \<Xi> \<xi>m1 \<xi>p1"
@@ -891,7 +297,7 @@ lemma value_sem_rename_mono_prog_rename_\<Xi>_\<xi>m1_\<xi>p1:
   apply (subst (asm) assoc_lookup.simps)+
   apply (clarsimp split: if_split_asm)
     apply (rule conjI; clarsimp; subst (asm) rename_def; clarsimp)
-    apply (clarsimp simp: val_wa_foldnb_0_def val_wa_foldnbp_def)
+    apply (clarsimp simp: val_wa_foldnb_def val_wa_foldnbp_def)
     apply (case_tac v; clarsimp)
     apply (case_tac z; clarsimp)
     apply (case_tac za; clarsimp)
@@ -930,7 +336,7 @@ lemma val_proc_env_matches_\<xi>m1_\<Xi>:
      apply (drule val_wa_length_preservation; simp?)
     apply (clarsimp simp: wordarray_put2_0_type_def abbreviated_type_defs)
     apply (drule val_wa_put2_preservation; simp?)
-   apply (clarsimp simp: wordarray_fold_no_break_0_type_def val_wa_foldnb_0_def)
+   apply (clarsimp simp: wordarray_fold_no_break_0_type_def val_wa_foldnb_def)
    apply (erule val.v_t_recordE)
    apply (erule val.v_t_r_consE; clarsimp)+
    apply (erule val.v_t_abstractE; clarsimp)
@@ -1221,7 +627,7 @@ lemma upd_val_wa_mapAccumnb_bod_corres:
   apply (erule conjE)+
   apply clarsimp
   apply (erule u_v_r_emptyE; clarsimp)
-  apply (erule u_v_t_prim_tE)
+  apply (erule u_v_t_primtE)
   apply clarsimp
   apply (drule_tac t = "lit_type _" in sym)+
   apply clarsimp
@@ -1418,18 +824,17 @@ lemma val_executes_fron_upd_wa_mapAccumnb_bod:
   done
 
 
-inductive_cases u_v_t_funE: "upd_val_rel \<Xi>' \<sigma> (UFunction f ts) v t r w"
-inductive_cases u_v_t_afunE: "upd_val_rel \<Xi>' \<sigma> (UAFunction f ts) v t r w"
+
 
 lemma wordarray_fold_no_break_upd_val:
   "\<And>K a b \<sigma> \<sigma>' \<tau>s aa a' v v' r w.
    \<lbrakk>list_all2 (kinding []) \<tau>s K; wordarray_fold_no_break_0_type = (K, a, b); 
     upd_val_rel \<Xi> \<sigma> aa a' (instantiate \<tau>s a) r w; 
-    upd_wa_foldnb_0 \<Xi> \<xi>0 (foldmap_funarg_type ''wordarray_fold_no_break_0'') (\<sigma>, aa) (\<sigma>', v)\<rbrakk>
-    \<Longrightarrow> (val_wa_foldnb_0 \<Xi> \<xi>m (foldmap_funarg_type ''wordarray_fold_no_break_0'') a' v' 
+    upd_wa_foldnb \<Xi> \<xi>0 (foldmap_funarg_type ''wordarray_fold_no_break_0'') (\<sigma>, aa) (\<sigma>', v)\<rbrakk>
+    \<Longrightarrow> (val_wa_foldnb \<Xi> \<xi>m (foldmap_funarg_type ''wordarray_fold_no_break_0'') a' v' 
           \<longrightarrow> (\<exists>r' w'. upd_val_rel \<Xi> \<sigma>' v v' (instantiate \<tau>s b) r' w' \<and> r' \<subseteq> r \<and> frame \<sigma> w \<sigma>' w')) \<and> 
-        Ex (val_wa_foldnb_0 \<Xi> \<xi>m (foldmap_funarg_type ''wordarray_fold_no_break_0'') a')"
-  apply (clarsimp simp: wordarray_fold_no_break_0_type_def upd_wa_foldnb_0_def)
+        Ex (val_wa_foldnb \<Xi> \<xi>m (foldmap_funarg_type ''wordarray_fold_no_break_0'') a')"
+  apply (clarsimp simp: wordarray_fold_no_break_0_type_def upd_wa_foldnb_def)
   apply (rotate_tac 6)
   apply (subst (asm) \<Xi>_def; clarsimp simp: wordarray_fold_no_break_0_type_def abbreviated_type_defs)
   apply (rename_tac rb wb rc)
@@ -1462,7 +867,7 @@ lemma wordarray_fold_no_break_upd_val:
   apply (frule_tac u = obsv in upd_val_rel_to_uval_typing(1))
   apply (drule_tac x = obsv in upd.uval_typing_unique_ptrs(1); simp?)
   apply clarsimp
-  apply (clarsimp simp: val_wa_foldnb_0_def)
+  apply (clarsimp simp: val_wa_foldnb_def)
   apply (erule impE; simp?)+
    apply (case_tac f; clarsimp; elim u_v_t_funE u_v_t_afunE; clarsimp)
   apply (erule impE, rule upd_val_rel_to_vval_typing(1); simp?)+
@@ -1551,7 +956,7 @@ lemma upd_proc_env_matches_ptrs_\<xi>1_\<Xi>:
     apply (drule upd_wa_length_preservation; simp)
    apply (clarsimp simp: wordarray_put2_0_type_def abbreviated_type_defs)
    apply (drule upd_wa_put2_preservation; simp)
-  apply (clarsimp simp: upd_wa_foldnb_0_preservation)
+  apply (clarsimp simp: upd_wa_foldnb_preservation)
   apply (clarsimp simp: upd_wa_mapAccumnb_preservation)
   done
 
